<?xml version="1.0"?>
<rdf:RDF xmlns="https://raw.githubusercontent.com/GTPB/Training_Course_Feedback/master/CFO.owl"
     xml:base="https://raw.githubusercontent.com/GTPB/Training_Course_Feedback/master/CFO.owl"
     xmlns:dc="http://purl.org/dc/elements/1.1"
     xmlns:owl="http://www.w3.org/2002/07/owl#"
     xmlns:rdf="http://www.w3.org/1999/02/22-rdf-syntax-ns#"
     xmlns:xml="http://www.w3.org/XML/1998/namespace"
     xmlns:xsd="http://www.w3.org/2001/XMLSchema#"
     xmlns:rdfs="http://www.w3.org/2000/01/rdf-schema#">
    <owl:Ontology rdf:about="https://raw.githubusercontent.com/GTPB/Training_Course_Feedback/master/CFO.owl">
        <dc:contributor>Alexandra Caetano</dc:contributor>
        <dc:contributor>Daniel Faria</dc:contributor>
        <dc:contributor>Pedro Fernandes</dc:contributor>
    </owl:Ontology>
    


    <!-- 
    ///////////////////////////////////////////////////////////////////////////////////////
    //
    // Annotation properties
    //
    ///////////////////////////////////////////////////////////////////////////////////////
     -->

    


    <!-- http://purl.org/dc/elements/1.1/contributor -->

    <owl:AnnotationProperty rdf:about="http://purl.org/dc/elements/1.1/contributor"/>
    


    <!-- 
    ///////////////////////////////////////////////////////////////////////////////////////
    //
    // Classes
    //
    ///////////////////////////////////////////////////////////////////////////////////////
     -->

    


    <!-- https://raw.githubusercontent.com/GTPB/Training_Course_Feedback/master/CFO.owl#announcement -->

    <owl:Class rdf:about="https://raw.githubusercontent.com/GTPB/Training_Course_Feedback/master/CFO.owl#announcement">
        <rdfs:subClassOf rdf:resource="https://raw.githubusercontent.com/GTPB/Training_Course_Feedback/master/CFO.owl#course_logistics"/>
        <rdfs:comment>A subject related to the announcement of a training course</rdfs:comment>
        <rdfs:label>Announcement</rdfs:label>
    </owl:Class>
    


    <!-- https://raw.githubusercontent.com/GTPB/Training_Course_Feedback/master/CFO.owl#background -->

    <owl:Class rdf:about="https://raw.githubusercontent.com/GTPB/Training_Course_Feedback/master/CFO.owl#background">
        <rdfs:subClassOf rdf:resource="https://raw.githubusercontent.com/GTPB/Training_Course_Feedback/master/CFO.owl#contextualization"/>
        <rdfs:comment>A comment about the background subject area of the participant</rdfs:comment>
        <rdfs:label>Background</rdfs:label>
    </owl:Class>
    


    <!-- https://raw.githubusercontent.com/GTPB/Training_Course_Feedback/master/CFO.owl#contextualization -->

    <owl:Class rdf:about="https://raw.githubusercontent.com/GTPB/Training_Course_Feedback/master/CFO.owl#contextualization">
        <rdfs:subClassOf rdf:resource="https://raw.githubusercontent.com/GTPB/Training_Course_Feedback/master/CFO.owl#participant_centred"/>
        <rdfs:comment>A subject related to the contextualization of the participant that attended a training course</rdfs:comment>
        <rdfs:label>Contextualization</rdfs:label>
    </owl:Class>
    


    <!-- https://raw.githubusercontent.com/GTPB/Training_Course_Feedback/master/CFO.owl#course_assessment -->

    <owl:Class rdf:about="https://raw.githubusercontent.com/GTPB/Training_Course_Feedback/master/CFO.owl#course_assessment">
        <rdfs:subClassOf rdf:resource="https://raw.githubusercontent.com/GTPB/Training_Course_Feedback/master/CFO.owl#participant_course_feedback_subject"/>
        <rdfs:comment xml:lang="en">A subject related to the functioning of a training course</rdfs:comment>
        <rdfs:label xml:lang="en">Course assessment</rdfs:label>
    </owl:Class>
    


    <!-- https://raw.githubusercontent.com/GTPB/Training_Course_Feedback/master/CFO.owl#course_design_and_delivery -->

    <owl:Class rdf:about="https://raw.githubusercontent.com/GTPB/Training_Course_Feedback/master/CFO.owl#course_design_and_delivery">
        <rdfs:subClassOf rdf:resource="https://raw.githubusercontent.com/GTPB/Training_Course_Feedback/master/CFO.owl#organization_centred"/>
        <rdfs:comment>A subject related to the design and implementation of a training course</rdfs:comment>
    </owl:Class>
    


    <!-- https://raw.githubusercontent.com/GTPB/Training_Course_Feedback/master/CFO.owl#course_logistics -->

    <owl:Class rdf:about="https://raw.githubusercontent.com/GTPB/Training_Course_Feedback/master/CFO.owl#course_logistics">
        <rdfs:subClassOf rdf:resource="https://raw.githubusercontent.com/GTPB/Training_Course_Feedback/master/CFO.owl#organization_centred"/>
        <rdfs:comment>A subject related to the logistic organization of a training course</rdfs:comment>
    </owl:Class>
    


    <!-- https://raw.githubusercontent.com/GTPB/Training_Course_Feedback/master/CFO.owl#course_preparation -->

    <owl:Class rdf:about="https://raw.githubusercontent.com/GTPB/Training_Course_Feedback/master/CFO.owl#course_preparation">
        <rdfs:subClassOf rdf:resource="https://raw.githubusercontent.com/GTPB/Training_Course_Feedback/master/CFO.owl#organization_centred"/>
        <rdfs:comment>A comment related to the preparation in advance of a training course</rdfs:comment>
        <rdfs:label>Course preparation</rdfs:label>
    </owl:Class>
    


    <!-- https://raw.githubusercontent.com/GTPB/Training_Course_Feedback/master/CFO.owl#expectations -->

    <owl:Class rdf:about="https://raw.githubusercontent.com/GTPB/Training_Course_Feedback/master/CFO.owl#expectations">
        <rdfs:subClassOf rdf:resource="https://raw.githubusercontent.com/GTPB/Training_Course_Feedback/master/CFO.owl#participant_centred"/>
        <rdfs:comment>A comment related to what the participant expects to learn in a training course and whether this expectations were fulfilled</rdfs:comment>
        <rdfs:label>Expectations</rdfs:label>
    </owl:Class>
    


    <!-- https://raw.githubusercontent.com/GTPB/Training_Course_Feedback/master/CFO.owl#extra_organization -->

    <owl:Class rdf:about="https://raw.githubusercontent.com/GTPB/Training_Course_Feedback/master/CFO.owl#extra_organization">
        <rdfs:subClassOf rdf:resource="https://raw.githubusercontent.com/GTPB/Training_Course_Feedback/master/CFO.owl#course_assessment"/>
        <rdfs:comment>A subject related to the organization of a training course out of the scope of the organization team</rdfs:comment>
        <rdfs:label>Extra-organization</rdfs:label>
    </owl:Class>
    


    <!-- https://raw.githubusercontent.com/GTPB/Training_Course_Feedback/master/CFO.owl#fee -->

    <owl:Class rdf:about="https://raw.githubusercontent.com/GTPB/Training_Course_Feedback/master/CFO.owl#fee">
        <rdfs:subClassOf rdf:resource="https://raw.githubusercontent.com/GTPB/Training_Course_Feedback/master/CFO.owl#organization_centred"/>
        <rdfs:comment>A comment related to the fee of the course</rdfs:comment>
        <rdfs:label>Fee</rdfs:label>
    </owl:Class>
    


    <!-- https://raw.githubusercontent.com/GTPB/Training_Course_Feedback/master/CFO.owl#future_course_theme -->

    <owl:Class rdf:about="https://raw.githubusercontent.com/GTPB/Training_Course_Feedback/master/CFO.owl#future_course_theme">
        <rdfs:subClassOf rdf:resource="https://raw.githubusercontent.com/GTPB/Training_Course_Feedback/master/CFO.owl#participant_course_feedback_subject"/>
        <rdfs:comment>Course theme about which the participant would be interested in learning in the near future</rdfs:comment>
        <rdfs:label>Future course theme</rdfs:label>
    </owl:Class>
    


    <!-- https://raw.githubusercontent.com/GTPB/Training_Course_Feedback/master/CFO.owl#impact -->

    <owl:Class rdf:about="https://raw.githubusercontent.com/GTPB/Training_Course_Feedback/master/CFO.owl#impact">
        <rdfs:subClassOf rdf:resource="https://raw.githubusercontent.com/GTPB/Training_Course_Feedback/master/CFO.owl#participant_centred"/>
        <rdfs:comment>A comment about the foreseeable impact of a training course to the participant professional life</rdfs:comment>
        <rdfs:label>Impact</rdfs:label>
    </owl:Class>
    


    <!-- https://raw.githubusercontent.com/GTPB/Training_Course_Feedback/master/CFO.owl#motivation -->

    <owl:Class rdf:about="https://raw.githubusercontent.com/GTPB/Training_Course_Feedback/master/CFO.owl#motivation">
        <rdfs:subClassOf rdf:resource="https://raw.githubusercontent.com/GTPB/Training_Course_Feedback/master/CFO.owl#contextualization"/>
        <rdfs:comment>A comment about the reasons that led the participant to attend a training course</rdfs:comment>
        <rdfs:label>Motivation</rdfs:label>
    </owl:Class>
    


    <!-- https://raw.githubusercontent.com/GTPB/Training_Course_Feedback/master/CFO.owl#organization_centred -->

    <owl:Class rdf:about="https://raw.githubusercontent.com/GTPB/Training_Course_Feedback/master/CFO.owl#organization_centred">
        <rdfs:subClassOf rdf:resource="https://raw.githubusercontent.com/GTPB/Training_Course_Feedback/master/CFO.owl#course_assessment"/>
        <rdfs:comment>A subject related to the organization of a training course in which the organization team is directly involved.</rdfs:comment>
        <rdfs:label>Organization centred</rdfs:label>
    </owl:Class>
    


    <!-- https://raw.githubusercontent.com/GTPB/Training_Course_Feedback/master/CFO.owl#participant_centred -->

    <owl:Class rdf:about="https://raw.githubusercontent.com/GTPB/Training_Course_Feedback/master/CFO.owl#participant_centred">
        <rdfs:subClassOf rdf:resource="https://raw.githubusercontent.com/GTPB/Training_Course_Feedback/master/CFO.owl#course_assessment"/>
        <rdfs:comment>A subject related to the participant attendance and experience in a training course</rdfs:comment>
        <rdfs:label>Participant-centred</rdfs:label>
    </owl:Class>
    


    <!-- https://raw.githubusercontent.com/GTPB/Training_Course_Feedback/master/CFO.owl#participant_course_feedback_subject -->

    <owl:Class rdf:about="https://raw.githubusercontent.com/GTPB/Training_Course_Feedback/master/CFO.owl#participant_course_feedback_subject">
        <rdfs:comment xml:lang="en">A subject related to a training course about which the participant provides feedback</rdfs:comment>
        <rdfs:label xml:lang="en">Participant course feedback subject</rdfs:label>
    </owl:Class>
    


    <!-- https://raw.githubusercontent.com/GTPB/Training_Course_Feedback/master/CFO.owl#participant_supoort -->

    <owl:Class rdf:about="https://raw.githubusercontent.com/GTPB/Training_Course_Feedback/master/CFO.owl#participant_supoort">
        <rdfs:subClassOf rdf:resource="https://raw.githubusercontent.com/GTPB/Training_Course_Feedback/master/CFO.owl#course_logistics"/>
        <rdfs:comment>A subject related to the support provided to the participant that attends a training course</rdfs:comment>
        <rdfs:label>Participant support</rdfs:label>
    </owl:Class>
    


    <!-- https://raw.githubusercontent.com/GTPB/Training_Course_Feedback/master/CFO.owl#previous_knowledge -->

    <owl:Class rdf:about="https://raw.githubusercontent.com/GTPB/Training_Course_Feedback/master/CFO.owl#previous_knowledge">
        <rdfs:subClassOf rdf:resource="https://raw.githubusercontent.com/GTPB/Training_Course_Feedback/master/CFO.owl#background"/>
        <rdfs:comment>A comment related to the participant&apos;s previous knowledge in the subject covered in a training course</rdfs:comment>
        <rdfs:label>Previous knowledge</rdfs:label>
    </owl:Class>
    


    <!-- https://raw.githubusercontent.com/GTPB/Training_Course_Feedback/master/CFO.owl#previous_skill -->

    <owl:Class rdf:about="https://raw.githubusercontent.com/GTPB/Training_Course_Feedback/master/CFO.owl#previous_skill">
        <rdfs:subClassOf rdf:resource="https://raw.githubusercontent.com/GTPB/Training_Course_Feedback/master/CFO.owl#background"/>
        <rdfs:comment>A comment related to the participant&apos; skills in the tools used in a training course</rdfs:comment>
        <rdfs:label>Previous skill</rdfs:label>
    </owl:Class>
    


    <!-- https://raw.githubusercontent.com/GTPB/Training_Course_Feedback/master/CFO.owl#publicity_source -->

    <owl:Class rdf:about="https://raw.githubusercontent.com/GTPB/Training_Course_Feedback/master/CFO.owl#publicity_source">
        <rdfs:subClassOf rdf:resource="https://raw.githubusercontent.com/GTPB/Training_Course_Feedback/master/CFO.owl#participant_course_feedback_subject"/>
        <rdfs:comment xml:lang="en">Source where the participant learned about the course</rdfs:comment>
        <rdfs:label xml:lang="en">Publicity source</rdfs:label>
    </owl:Class>
    


    <!-- https://raw.githubusercontent.com/GTPB/Training_Course_Feedback/master/CFO.owl#recommendation -->

    <owl:Class rdf:about="https://raw.githubusercontent.com/GTPB/Training_Course_Feedback/master/CFO.owl#recommendation">
        <rdfs:subClassOf rdf:resource="https://raw.githubusercontent.com/GTPB/Training_Course_Feedback/master/CFO.owl#participant_centred"/>
        <rdfs:comment>A comment related to the pariticipant’s willingness to recommend the course</rdfs:comment>
        <rdfs:label>Recommendation</rdfs:label>
    </owl:Class>
    


    <!-- https://raw.githubusercontent.com/GTPB/Training_Course_Feedback/master/CFO.owl#registration -->

    <owl:Class rdf:about="https://raw.githubusercontent.com/GTPB/Training_Course_Feedback/master/CFO.owl#registration">
        <rdfs:subClassOf rdf:resource="https://raw.githubusercontent.com/GTPB/Training_Course_Feedback/master/CFO.owl#course_logistics"/>
        <rdfs:comment>A subject related to the registration of a training course</rdfs:comment>
        <rdfs:label>Registration</rdfs:label>
    </owl:Class>
    


    <!-- https://raw.githubusercontent.com/GTPB/Training_Course_Feedback/master/CFO.owl#statement -->

    <owl:Class rdf:about="https://raw.githubusercontent.com/GTPB/Training_Course_Feedback/master/CFO.owl#statement">
        <rdfs:subClassOf rdf:resource="https://raw.githubusercontent.com/GTPB/Training_Course_Feedback/master/CFO.owl#participant_centred"/>
        <rdfs:comment>Comment related to what the participant perceived to have learned in a training course</rdfs:comment>
        <rdfs:label>Statement</rdfs:label>
    </owl:Class>
    


    <!-- https://raw.githubusercontent.com/GTPB/Training_Course_Feedback/master/CFO.owl#testimonial -->

    <owl:Class rdf:about="https://raw.githubusercontent.com/GTPB/Training_Course_Feedback/master/CFO.owl#testimonial">
        <rdfs:subClassOf rdf:resource="https://raw.githubusercontent.com/GTPB/Training_Course_Feedback/master/CFO.owl#participant_centred"/>
        <rdfs:comment>A comment related to the participant&apos; s overall experience and general appreciation about a training course</rdfs:comment>
        <rdfs:label>Testimonial</rdfs:label>
    </owl:Class>
    


    <!-- https://raw.githubusercontent.com/GTPB/Training_Course_Feedback/master/CFO.owl#title -->

    <owl:Class rdf:about="https://raw.githubusercontent.com/GTPB/Training_Course_Feedback/master/CFO.owl#title">
        <rdfs:subClassOf rdf:resource="https://raw.githubusercontent.com/GTPB/Training_Course_Feedback/master/CFO.owl#organization_centred"/>
        <rdfs:comment>A comment related to the name of the course</rdfs:comment>
    </owl:Class>
</rdf:RDF>



<!-- Generated by the OWL API (version 4.5.6.2018-09-06T00:27:41Z) https://github.com/owlcs/owlapi -->

