<?xml version="1.0"?>
<rdf:RDF xmlns="https://raw.githubusercontent.com/GTPB/Training_Course_Feedback/master/CFO.owl"
     xml:base="https://raw.githubusercontent.com/GTPB/Training_Course_Feedback/master/CFO.owl"
     xmlns:dc="http://purl.org/dc/elements/1.1"
     xmlns:owl="http://www.w3.org/2002/07/owl#"
     xmlns:rdf="http://www.w3.org/1999/02/22-rdf-syntax-ns#"
     xmlns:xml="http://www.w3.org/XML/1998/namespace"
     xmlns:xsd="http://www.w3.org/2001/XMLSchema#"
     xmlns:rdfs="http://www.w3.org/2000/01/rdf-schema#">
    <owl:Ontology rdf:about="https://raw.githubusercontent.com/GTPB/Training_Course_Feedback/master/CFO.owl">
        <dc:contributor>Alexandra Caetano</dc:contributor>
        <dc:contributor>Daniel Faria</dc:contributor>
        <dc:contributor>Pedro Fernandes</dc:contributor>
    </owl:Ontology>
    


    <!-- 
    ///////////////////////////////////////////////////////////////////////////////////////
    //
    // Annotation properties
    //
    ///////////////////////////////////////////////////////////////////////////////////////
     -->

    


    <!-- http://purl.org/dc/elements/1.1/contributor -->

    <owl:AnnotationProperty rdf:about="http://purl.org/dc/elements/1.1/contributor"/>
    


    <!-- 
    ///////////////////////////////////////////////////////////////////////////////////////
    //
    // Classes
    //
    ///////////////////////////////////////////////////////////////////////////////////////
     -->

    


    <!-- https://raw.githubusercontent.com/GTPB/Training_Course_Feedback/master/CFO.owl#accessibility -->

    <owl:Class rdf:about="https://raw.githubusercontent.com/GTPB/Training_Course_Feedback/master/CFO.owl#accessibility">
        <rdfs:subClassOf rdf:resource="https://raw.githubusercontent.com/GTPB/Training_Course_Feedback/master/CFO.owl#tag_descriptor"/>
    </owl:Class>
    


    <!-- https://raw.githubusercontent.com/GTPB/Training_Course_Feedback/master/CFO.owl#accreditation -->

    <owl:Class rdf:about="https://raw.githubusercontent.com/GTPB/Training_Course_Feedback/master/CFO.owl#accreditation">
        <rdfs:subClassOf rdf:resource="https://raw.githubusercontent.com/GTPB/Training_Course_Feedback/master/CFO.owl#materials"/>
        <rdfs:comment>A comment related to the formal documentation accredited in a training course (e.g. certificates of attendance, diplomas)</rdfs:comment>
        <rdfs:label>Accreditation</rdfs:label>
    </owl:Class>
    


    <!-- https://raw.githubusercontent.com/GTPB/Training_Course_Feedback/master/CFO.owl#accuracy -->

    <owl:Class rdf:about="https://raw.githubusercontent.com/GTPB/Training_Course_Feedback/master/CFO.owl#accuracy">
        <rdfs:subClassOf rdf:resource="https://raw.githubusercontent.com/GTPB/Training_Course_Feedback/master/CFO.owl#tag_descriptor"/>
    </owl:Class>
    


    <!-- https://raw.githubusercontent.com/GTPB/Training_Course_Feedback/master/CFO.owl#activity -->

    <owl:Class rdf:about="https://raw.githubusercontent.com/GTPB/Training_Course_Feedback/master/CFO.owl#activity">
        <rdfs:subClassOf rdf:resource="https://raw.githubusercontent.com/GTPB/Training_Course_Feedback/master/CFO.owl#structure"/>
        <rdfs:subClassOf rdf:resource="https://raw.githubusercontent.com/GTPB/Training_Course_Feedback/master/CFO.owl#time_management"/>
        <rdfs:comment>A comment related to the activities performed in the course</rdfs:comment>
        <rdfs:label>Activity</rdfs:label>
    </owl:Class>
    


    <!-- https://raw.githubusercontent.com/GTPB/Training_Course_Feedback/master/CFO.owl#adequacy -->

    <owl:Class rdf:about="https://raw.githubusercontent.com/GTPB/Training_Course_Feedback/master/CFO.owl#adequacy">
        <rdfs:subClassOf rdf:resource="https://raw.githubusercontent.com/GTPB/Training_Course_Feedback/master/CFO.owl#tag_descriptor"/>
    </owl:Class>
    


    <!-- https://raw.githubusercontent.com/GTPB/Training_Course_Feedback/master/CFO.owl#admission -->

    <owl:Class rdf:about="https://raw.githubusercontent.com/GTPB/Training_Course_Feedback/master/CFO.owl#admission">
        <rdfs:subClassOf rdf:resource="https://raw.githubusercontent.com/GTPB/Training_Course_Feedback/master/CFO.owl#registration"/>
        <rdfs:comment>A comment related to the acceptance process and procedures for a training course</rdfs:comment>
        <rdfs:label>Admission</rdfs:label>
    </owl:Class>
    


    <!-- https://raw.githubusercontent.com/GTPB/Training_Course_Feedback/master/CFO.owl#after_course_activities -->

    <owl:Class rdf:about="https://raw.githubusercontent.com/GTPB/Training_Course_Feedback/master/CFO.owl#after_course_activities">
        <rdfs:subClassOf rdf:resource="https://raw.githubusercontent.com/GTPB/Training_Course_Feedback/master/CFO.owl#social"/>
        <rdfs:comment>A comment related to the promotion and organization of local and/or online activities after the end date of a training course</rdfs:comment>
        <rdfs:label>After-course activities</rdfs:label>
    </owl:Class>
    


    <!-- https://raw.githubusercontent.com/GTPB/Training_Course_Feedback/master/CFO.owl#air_quality -->

    <owl:Class rdf:about="https://raw.githubusercontent.com/GTPB/Training_Course_Feedback/master/CFO.owl#air_quality">
        <rdfs:subClassOf rdf:resource="https://raw.githubusercontent.com/GTPB/Training_Course_Feedback/master/CFO.owl#climate"/>
        <rdfs:comment>A comment related to the air quality of the training room where a training course takes place</rdfs:comment>
        <rdfs:label>Air quality</rdfs:label>
    </owl:Class>
    


    <!-- https://raw.githubusercontent.com/GTPB/Training_Course_Feedback/master/CFO.owl#announcement -->

    <owl:Class rdf:about="https://raw.githubusercontent.com/GTPB/Training_Course_Feedback/master/CFO.owl#announcement">
        <rdfs:subClassOf rdf:resource="https://raw.githubusercontent.com/GTPB/Training_Course_Feedback/master/CFO.owl#course_logistics"/>
        <rdfs:comment>A subject related to the announcement of a training course</rdfs:comment>
        <rdfs:label>Announcement</rdfs:label>
    </owl:Class>
    


    <!-- https://raw.githubusercontent.com/GTPB/Training_Course_Feedback/master/CFO.owl#answer_key -->

    <owl:Class rdf:about="https://raw.githubusercontent.com/GTPB/Training_Course_Feedback/master/CFO.owl#answer_key">
        <rdfs:subClassOf rdf:resource="https://raw.githubusercontent.com/GTPB/Training_Course_Feedback/master/CFO.owl#auxiliary"/>
        <rdfs:comment>A comment related to the use of answer keys to explicit the results and solutions of the exercises and assignments in a training course</rdfs:comment>
        <rdfs:label>Answer key</rdfs:label>
    </owl:Class>
    


    <!-- https://raw.githubusercontent.com/GTPB/Training_Course_Feedback/master/CFO.owl#application -->

    <owl:Class rdf:about="https://raw.githubusercontent.com/GTPB/Training_Course_Feedback/master/CFO.owl#application">
        <rdfs:subClassOf rdf:resource="https://raw.githubusercontent.com/GTPB/Training_Course_Feedback/master/CFO.owl#registration"/>
        <rdfs:comment>A comment related to the application process and procedures of a training course</rdfs:comment>
        <rdfs:label>Application</rdfs:label>
    </owl:Class>
    


    <!-- https://raw.githubusercontent.com/GTPB/Training_Course_Feedback/master/CFO.owl#approach -->

    <owl:Class rdf:about="https://raw.githubusercontent.com/GTPB/Training_Course_Feedback/master/CFO.owl#approach">
        <rdfs:subClassOf rdf:resource="https://raw.githubusercontent.com/GTPB/Training_Course_Feedback/master/CFO.owl#instructional_methodology"/>
        <rdfs:comment>A comment related to the approach selected to cover the theme of a training course</rdfs:comment>
        <rdfs:label>Approach</rdfs:label>
    </owl:Class>
    


    <!-- https://raw.githubusercontent.com/GTPB/Training_Course_Feedback/master/CFO.owl#assessment_instruments -->

    <owl:Class rdf:about="https://raw.githubusercontent.com/GTPB/Training_Course_Feedback/master/CFO.owl#assessment_instruments">
        <rdfs:subClassOf rdf:resource="https://raw.githubusercontent.com/GTPB/Training_Course_Feedback/master/CFO.owl#strategies"/>
        <rdfs:comment>A subject related to the assessment of the participant&apos;s learning process in a training course</rdfs:comment>
        <rdfs:label>Assessment instruments</rdfs:label>
    </owl:Class>
    


    <!-- https://raw.githubusercontent.com/GTPB/Training_Course_Feedback/master/CFO.owl#assignments -->

    <owl:Class rdf:about="https://raw.githubusercontent.com/GTPB/Training_Course_Feedback/master/CFO.owl#assignments">
        <rdfs:subClassOf rdf:resource="https://raw.githubusercontent.com/GTPB/Training_Course_Feedback/master/CFO.owl#instructional_instruments"/>
        <rdfs:comment>A comment related to the type of assignments and tasks proposed in a training course (e.g. project, problem-solving, etc)</rdfs:comment>
        <rdfs:label>Assignments</rdfs:label>
    </owl:Class>
    


    <!-- https://raw.githubusercontent.com/GTPB/Training_Course_Feedback/master/CFO.owl#audience -->

    <owl:Class rdf:about="https://raw.githubusercontent.com/GTPB/Training_Course_Feedback/master/CFO.owl#audience">
        <rdfs:subClassOf rdf:resource="https://raw.githubusercontent.com/GTPB/Training_Course_Feedback/master/CFO.owl#course_design_and_delivery"/>
        <rdfs:comment>A comment about the target audience of a training course</rdfs:comment>
        <rdfs:label>Audience</rdfs:label>
    </owl:Class>
    


    <!-- https://raw.githubusercontent.com/GTPB/Training_Course_Feedback/master/CFO.owl#autonomy -->

    <owl:Class rdf:about="https://raw.githubusercontent.com/GTPB/Training_Course_Feedback/master/CFO.owl#autonomy">
        <rdfs:subClassOf rdf:resource="https://raw.githubusercontent.com/GTPB/Training_Course_Feedback/master/CFO.owl#self_assessment"/>
        <rdfs:comment>The participant believes that gained independence and autonomy (i.e. competence) in the subject theme addressed in a training course</rdfs:comment>
        <rdfs:label>Autonomy</rdfs:label>
    </owl:Class>
    


    <!-- https://raw.githubusercontent.com/GTPB/Training_Course_Feedback/master/CFO.owl#auxiliary -->

    <owl:Class rdf:about="https://raw.githubusercontent.com/GTPB/Training_Course_Feedback/master/CFO.owl#auxiliary">
        <rdfs:subClassOf rdf:resource="https://raw.githubusercontent.com/GTPB/Training_Course_Feedback/master/CFO.owl#instructional_instruments"/>
        <rdfs:comment>A subject related to the use of auxiliary instruments to support the learning experience in a training course</rdfs:comment>
        <rdfs:label>Auxiliary</rdfs:label>
    </owl:Class>
    


    <!-- https://raw.githubusercontent.com/GTPB/Training_Course_Feedback/master/CFO.owl#background -->

    <owl:Class rdf:about="https://raw.githubusercontent.com/GTPB/Training_Course_Feedback/master/CFO.owl#background">
        <rdfs:subClassOf rdf:resource="https://raw.githubusercontent.com/GTPB/Training_Course_Feedback/master/CFO.owl#contextualization"/>
        <rdfs:comment>A comment about the background subject area of the participant</rdfs:comment>
        <rdfs:label>Background</rdfs:label>
    </owl:Class>
    


    <!-- https://raw.githubusercontent.com/GTPB/Training_Course_Feedback/master/CFO.owl#badge -->

    <owl:Class rdf:about="https://raw.githubusercontent.com/GTPB/Training_Course_Feedback/master/CFO.owl#badge">
        <rdfs:subClassOf rdf:resource="https://raw.githubusercontent.com/GTPB/Training_Course_Feedback/master/CFO.owl#participant_support"/>
        <rdfs:comment>A comment related to the provision of badges identifying the participants (e.g. name, affiliation, interests) in a training room</rdfs:comment>
        <rdfs:label>Badge</rdfs:label>
    </owl:Class>
    


    <!-- https://raw.githubusercontent.com/GTPB/Training_Course_Feedback/master/CFO.owl#balance -->

    <owl:Class rdf:about="https://raw.githubusercontent.com/GTPB/Training_Course_Feedback/master/CFO.owl#balance">
        <rdfs:subClassOf rdf:resource="https://raw.githubusercontent.com/GTPB/Training_Course_Feedback/master/CFO.owl#tag_descriptor"/>
    </owl:Class>
    


    <!-- https://raw.githubusercontent.com/GTPB/Training_Course_Feedback/master/CFO.owl#bottom_up -->

    <owl:Class rdf:about="https://raw.githubusercontent.com/GTPB/Training_Course_Feedback/master/CFO.owl#bottom_up">
        <rdfs:subClassOf rdf:resource="https://raw.githubusercontent.com/GTPB/Training_Course_Feedback/master/CFO.owl#approach"/>
        <rdfs:comment>A comment related to the approach of sequential progressing of a subject theme from the small details to the broaden concepts in a training course</rdfs:comment>
        <rdfs:label>Bottom-up approach</rdfs:label>
    </owl:Class>
    


    <!-- https://raw.githubusercontent.com/GTPB/Training_Course_Feedback/master/CFO.owl#break -->

    <owl:Class rdf:about="https://raw.githubusercontent.com/GTPB/Training_Course_Feedback/master/CFO.owl#break">
        <rdfs:subClassOf rdf:resource="https://raw.githubusercontent.com/GTPB/Training_Course_Feedback/master/CFO.owl#activity"/>
        <rdfs:comment>A comment related to the break periods of a training course</rdfs:comment>
        <rdfs:label>Break</rdfs:label>
    </owl:Class>
    


    <!-- https://raw.githubusercontent.com/GTPB/Training_Course_Feedback/master/CFO.owl#call -->

    <owl:Class rdf:about="https://raw.githubusercontent.com/GTPB/Training_Course_Feedback/master/CFO.owl#call">
        <rdfs:subClassOf rdf:resource="https://raw.githubusercontent.com/GTPB/Training_Course_Feedback/master/CFO.owl#registration"/>
        <rdfs:comment>A comment related to the application call for a training course</rdfs:comment>
        <rdfs:label>Call</rdfs:label>
    </owl:Class>
    


    <!-- https://raw.githubusercontent.com/GTPB/Training_Course_Feedback/master/CFO.owl#catering -->

    <owl:Class rdf:about="https://raw.githubusercontent.com/GTPB/Training_Course_Feedback/master/CFO.owl#catering">
        <rdfs:subClassOf rdf:resource="https://raw.githubusercontent.com/GTPB/Training_Course_Feedback/master/CFO.owl#participant_support"/>
        <rdfs:comment>A comment related to the provision of the coffee-breaks and lunch break in a training course</rdfs:comment>
        <rdfs:label>Catering</rdfs:label>
    </owl:Class>
    


    <!-- https://raw.githubusercontent.com/GTPB/Training_Course_Feedback/master/CFO.owl#challenging -->

    <owl:Class rdf:about="https://raw.githubusercontent.com/GTPB/Training_Course_Feedback/master/CFO.owl#challenging">
        <rdfs:subClassOf rdf:resource="https://raw.githubusercontent.com/GTPB/Training_Course_Feedback/master/CFO.owl#testimonial"/>
        <rdfs:comment>The course was challenging</rdfs:comment>
        <rdfs:label>Challenging</rdfs:label>
    </owl:Class>
    


    <!-- https://raw.githubusercontent.com/GTPB/Training_Course_Feedback/master/CFO.owl#city_tour -->

    <owl:Class rdf:about="https://raw.githubusercontent.com/GTPB/Training_Course_Feedback/master/CFO.owl#city_tour">
        <rdfs:subClassOf rdf:resource="https://raw.githubusercontent.com/GTPB/Training_Course_Feedback/master/CFO.owl#social"/>
        <rdfs:comment>A comment related to the promotion and organization of a guided tour to local places during the timespan of a training course</rdfs:comment>
        <rdfs:label>City tour</rdfs:label>
    </owl:Class>
    


    <!-- https://raw.githubusercontent.com/GTPB/Training_Course_Feedback/master/CFO.owl#clarity -->

    <owl:Class rdf:about="https://raw.githubusercontent.com/GTPB/Training_Course_Feedback/master/CFO.owl#clarity">
        <rdfs:subClassOf rdf:resource="https://raw.githubusercontent.com/GTPB/Training_Course_Feedback/master/CFO.owl#tag_descriptor"/>
    </owl:Class>
    


    <!-- https://raw.githubusercontent.com/GTPB/Training_Course_Feedback/master/CFO.owl#class_size -->

    <owl:Class rdf:about="https://raw.githubusercontent.com/GTPB/Training_Course_Feedback/master/CFO.owl#class_size">
        <rdfs:subClassOf rdf:resource="https://raw.githubusercontent.com/GTPB/Training_Course_Feedback/master/CFO.owl#course_design_and_delivery"/>
        <rdfs:comment>A comment related to the number of participants in a training course</rdfs:comment>
        <rdfs:label>Class size</rdfs:label>
    </owl:Class>
    


    <!-- https://raw.githubusercontent.com/GTPB/Training_Course_Feedback/master/CFO.owl#climate -->

    <owl:Class rdf:about="https://raw.githubusercontent.com/GTPB/Training_Course_Feedback/master/CFO.owl#climate">
        <rdfs:subClassOf rdf:resource="https://raw.githubusercontent.com/GTPB/Training_Course_Feedback/master/CFO.owl#training_room"/>
        <rdfs:comment>A comment related to the environmental conditions of the training room where a training course takes place</rdfs:comment>
        <rdfs:label>Climate</rdfs:label>
    </owl:Class>
    


    <!-- https://raw.githubusercontent.com/GTPB/Training_Course_Feedback/master/CFO.owl#communication -->

    <owl:Class rdf:about="https://raw.githubusercontent.com/GTPB/Training_Course_Feedback/master/CFO.owl#communication">
        <rdfs:subClassOf rdf:resource="https://raw.githubusercontent.com/GTPB/Training_Course_Feedback/master/CFO.owl#educational_content"/>
        <rdfs:comment>A comment related to the communication of the content in a training course</rdfs:comment>
        <rdfs:label>Communication</rdfs:label>
    </owl:Class>
    


    <!-- https://raw.githubusercontent.com/GTPB/Training_Course_Feedback/master/CFO.owl#complete -->

    <owl:Class rdf:about="https://raw.githubusercontent.com/GTPB/Training_Course_Feedback/master/CFO.owl#complete">
        <rdfs:subClassOf rdf:resource="https://raw.githubusercontent.com/GTPB/Training_Course_Feedback/master/CFO.owl#testimonial"/>
        <rdfs:comment>The course was complete</rdfs:comment>
        <rdfs:label>Complete</rdfs:label>
    </owl:Class>
    


    <!-- https://raw.githubusercontent.com/GTPB/Training_Course_Feedback/master/CFO.owl#computers -->

    <owl:Class rdf:about="https://raw.githubusercontent.com/GTPB/Training_Course_Feedback/master/CFO.owl#computers">
        <rdfs:subClassOf rdf:resource="https://raw.githubusercontent.com/GTPB/Training_Course_Feedback/master/CFO.owl#equipment"/>
        <rdfs:comment>A comment related to the computers in a training course</rdfs:comment>
        <rdfs:label>Computers</rdfs:label>
    </owl:Class>
    


    <!-- https://raw.githubusercontent.com/GTPB/Training_Course_Feedback/master/CFO.owl#confidence -->

    <owl:Class rdf:about="https://raw.githubusercontent.com/GTPB/Training_Course_Feedback/master/CFO.owl#confidence">
        <rdfs:subClassOf rdf:resource="https://raw.githubusercontent.com/GTPB/Training_Course_Feedback/master/CFO.owl#self_assessment"/>
        <rdfs:comment>The participant believes that gained confidence in the application of the skills adressed in a training course</rdfs:comment>
        <rdfs:label>Confidence</rdfs:label>
    </owl:Class>
    


    <!-- https://raw.githubusercontent.com/GTPB/Training_Course_Feedback/master/CFO.owl#confirmation -->

    <owl:Class rdf:about="https://raw.githubusercontent.com/GTPB/Training_Course_Feedback/master/CFO.owl#confirmation">
        <rdfs:subClassOf rdf:resource="https://raw.githubusercontent.com/GTPB/Training_Course_Feedback/master/CFO.owl#admission"/>
        <rdfs:comment>A comment related to the communication to the participant that he/she was admitted to a training course.</rdfs:comment>
        <rdfs:label>Confirmation</rdfs:label>
    </owl:Class>
    


    <!-- https://raw.githubusercontent.com/GTPB/Training_Course_Feedback/master/CFO.owl#connectivity -->

    <owl:Class rdf:about="https://raw.githubusercontent.com/GTPB/Training_Course_Feedback/master/CFO.owl#connectivity">
        <rdfs:subClassOf rdf:resource="https://raw.githubusercontent.com/GTPB/Training_Course_Feedback/master/CFO.owl#tag_descriptor"/>
    </owl:Class>
    


    <!-- https://raw.githubusercontent.com/GTPB/Training_Course_Feedback/master/CFO.owl#content_scheme -->

    <owl:Class rdf:about="https://raw.githubusercontent.com/GTPB/Training_Course_Feedback/master/CFO.owl#content_scheme">
        <rdfs:subClassOf rdf:resource="https://raw.githubusercontent.com/GTPB/Training_Course_Feedback/master/CFO.owl#educational_content"/>
        <rdfs:comment>A comment related to the organization and structure of the content delivered in a training course</rdfs:comment>
        <rdfs:label>Content scheme</rdfs:label>
    </owl:Class>
    


    <!-- https://raw.githubusercontent.com/GTPB/Training_Course_Feedback/master/CFO.owl#content_type -->

    <owl:Class rdf:about="https://raw.githubusercontent.com/GTPB/Training_Course_Feedback/master/CFO.owl#content_type">
        <rdfs:subClassOf rdf:resource="https://raw.githubusercontent.com/GTPB/Training_Course_Feedback/master/CFO.owl#educational_content"/>
        <rdfs:comment>A subject related to the type of educational content delivered in a training course</rdfs:comment>
        <rdfs:label>Content type</rdfs:label>
    </owl:Class>
    


    <!-- https://raw.githubusercontent.com/GTPB/Training_Course_Feedback/master/CFO.owl#context -->

    <owl:Class rdf:about="https://raw.githubusercontent.com/GTPB/Training_Course_Feedback/master/CFO.owl#context">
        <rdfs:subClassOf rdf:resource="https://raw.githubusercontent.com/GTPB/Training_Course_Feedback/master/CFO.owl#educational_content"/>
        <rdfs:comment>A comment related to the context preferred to illustrate the theme covered in a training course</rdfs:comment>
        <rdfs:label>Context</rdfs:label>
    </owl:Class>
    


    <!-- https://raw.githubusercontent.com/GTPB/Training_Course_Feedback/master/CFO.owl#contextualization -->

    <owl:Class rdf:about="https://raw.githubusercontent.com/GTPB/Training_Course_Feedback/master/CFO.owl#contextualization">
        <rdfs:subClassOf rdf:resource="https://raw.githubusercontent.com/GTPB/Training_Course_Feedback/master/CFO.owl#pre_course"/>
        <rdfs:comment>A subject related to the participant&apos;s context prior to the start date of a training course</rdfs:comment>
        <rdfs:label>Contextualization</rdfs:label>
    </owl:Class>
    


    <!-- https://raw.githubusercontent.com/GTPB/Training_Course_Feedback/master/CFO.owl#coordination -->

    <owl:Class rdf:about="https://raw.githubusercontent.com/GTPB/Training_Course_Feedback/master/CFO.owl#coordination">
        <rdfs:subClassOf rdf:resource="https://raw.githubusercontent.com/GTPB/Training_Course_Feedback/master/CFO.owl#tag_descriptor"/>
    </owl:Class>
    


    <!-- https://raw.githubusercontent.com/GTPB/Training_Course_Feedback/master/CFO.owl#copy_pasting -->

    <owl:Class rdf:about="https://raw.githubusercontent.com/GTPB/Training_Course_Feedback/master/CFO.owl#copy_pasting">
        <rdfs:subClassOf rdf:resource="https://raw.githubusercontent.com/GTPB/Training_Course_Feedback/master/CFO.owl#implementation"/>
        <rdfs:comment>A comment related to the use of the copy and paste technique to provide instruction in a training course</rdfs:comment>
        <rdfs:label>Copy pasting</rdfs:label>
    </owl:Class>
    


    <!-- https://raw.githubusercontent.com/GTPB/Training_Course_Feedback/master/CFO.owl#course_assessment -->

    <owl:Class rdf:about="https://raw.githubusercontent.com/GTPB/Training_Course_Feedback/master/CFO.owl#course_assessment">
        <rdfs:subClassOf rdf:resource="https://raw.githubusercontent.com/GTPB/Training_Course_Feedback/master/CFO.owl#participant_course_feedback_subject"/>
        <rdfs:comment xml:lang="en">A subject related to the functioning of a training course</rdfs:comment>
        <rdfs:label xml:lang="en">Course assessment</rdfs:label>
    </owl:Class>
    


    <!-- https://raw.githubusercontent.com/GTPB/Training_Course_Feedback/master/CFO.owl#course_design_and_delivery -->

    <owl:Class rdf:about="https://raw.githubusercontent.com/GTPB/Training_Course_Feedback/master/CFO.owl#course_design_and_delivery">
        <rdfs:subClassOf rdf:resource="https://raw.githubusercontent.com/GTPB/Training_Course_Feedback/master/CFO.owl#organization_centred"/>
        <rdfs:comment>A subject related to the design and implementation of a training course</rdfs:comment>
        <rdfs:label>Course design and delivery</rdfs:label>
    </owl:Class>
    


    <!-- https://raw.githubusercontent.com/GTPB/Training_Course_Feedback/master/CFO.owl#course_logistics -->

    <owl:Class rdf:about="https://raw.githubusercontent.com/GTPB/Training_Course_Feedback/master/CFO.owl#course_logistics">
        <rdfs:subClassOf rdf:resource="https://raw.githubusercontent.com/GTPB/Training_Course_Feedback/master/CFO.owl#organization_centred"/>
        <rdfs:comment>A subject related to the logistic organization of a training course</rdfs:comment>
        <rdfs:label>Course logistics</rdfs:label>
    </owl:Class>
    


    <!-- https://raw.githubusercontent.com/GTPB/Training_Course_Feedback/master/CFO.owl#course_preparation -->

    <owl:Class rdf:about="https://raw.githubusercontent.com/GTPB/Training_Course_Feedback/master/CFO.owl#course_preparation">
        <rdfs:subClassOf rdf:resource="https://raw.githubusercontent.com/GTPB/Training_Course_Feedback/master/CFO.owl#organization_centred"/>
        <rdfs:comment>A comment related to the prior preparation to the deployment of a training course</rdfs:comment>
        <rdfs:label>Course preparation</rdfs:label>
    </owl:Class>
    


    <!-- https://raw.githubusercontent.com/GTPB/Training_Course_Feedback/master/CFO.owl#course_type -->

    <owl:Class rdf:about="https://raw.githubusercontent.com/GTPB/Training_Course_Feedback/master/CFO.owl#course_type">
        <rdfs:subClassOf rdf:resource="https://raw.githubusercontent.com/GTPB/Training_Course_Feedback/master/CFO.owl#course_design_and_delivery"/>
        <rdfs:comment>A comment related to the format of a training course (i.e. practical, theoretical, etc)</rdfs:comment>
        <rdfs:label>Course type</rdfs:label>
    </owl:Class>
    


    <!-- https://raw.githubusercontent.com/GTPB/Training_Course_Feedback/master/CFO.owl#coverage -->

    <owl:Class rdf:about="https://raw.githubusercontent.com/GTPB/Training_Course_Feedback/master/CFO.owl#coverage">
        <rdfs:subClassOf rdf:resource="https://raw.githubusercontent.com/GTPB/Training_Course_Feedback/master/CFO.owl#course_design_and_delivery"/>
        <rdfs:comment>A comment related to the topic coverage of a training course</rdfs:comment>
        <rdfs:label>Topic coverage</rdfs:label>
    </owl:Class>
    


    <!-- https://raw.githubusercontent.com/GTPB/Training_Course_Feedback/master/CFO.owl#criteria -->

    <owl:Class rdf:about="https://raw.githubusercontent.com/GTPB/Training_Course_Feedback/master/CFO.owl#criteria">
        <rdfs:subClassOf rdf:resource="https://raw.githubusercontent.com/GTPB/Training_Course_Feedback/master/CFO.owl#admission"/>
        <rdfs:comment>A comment related to the criteria selected to admit the participants in a training course</rdfs:comment>
        <rdfs:label>Admission criteria</rdfs:label>
    </owl:Class>
    


    <!-- https://raw.githubusercontent.com/GTPB/Training_Course_Feedback/master/CFO.owl#critical_thinking -->

    <owl:Class rdf:about="https://raw.githubusercontent.com/GTPB/Training_Course_Feedback/master/CFO.owl#critical_thinking">
        <rdfs:subClassOf rdf:resource="https://raw.githubusercontent.com/GTPB/Training_Course_Feedback/master/CFO.owl#self_assessment"/>
        <rdfs:comment>The participant believes that gained capability of understand and discuss the concepts explored in a training course</rdfs:comment>
        <rdfs:label>Critical thinking</rdfs:label>
    </owl:Class>
    


    <!-- https://raw.githubusercontent.com/GTPB/Training_Course_Feedback/master/CFO.owl#data_file -->

    <owl:Class rdf:about="https://raw.githubusercontent.com/GTPB/Training_Course_Feedback/master/CFO.owl#data_file">
        <rdfs:subClassOf rdf:resource="https://raw.githubusercontent.com/GTPB/Training_Course_Feedback/master/CFO.owl#materials"/>
        <rdfs:comment>A comment related to the physical files which contain the data delivered in a training course</rdfs:comment>
        <rdfs:label>Data file</rdfs:label>
    </owl:Class>
    


    <!-- https://raw.githubusercontent.com/GTPB/Training_Course_Feedback/master/CFO.owl#databases -->

    <owl:Class rdf:about="https://raw.githubusercontent.com/GTPB/Training_Course_Feedback/master/CFO.owl#databases">
        <rdfs:subClassOf rdf:resource="https://raw.githubusercontent.com/GTPB/Training_Course_Feedback/master/CFO.owl#tools"/>
        <rdfs:comment>A comment related to the databases selected as platforms to use in a training course</rdfs:comment>
        <rdfs:label>Databases</rdfs:label>
    </owl:Class>
    


    <!-- https://raw.githubusercontent.com/GTPB/Training_Course_Feedback/master/CFO.owl#dataset -->

    <owl:Class rdf:about="https://raw.githubusercontent.com/GTPB/Training_Course_Feedback/master/CFO.owl#dataset">
        <rdfs:subClassOf rdf:resource="https://raw.githubusercontent.com/GTPB/Training_Course_Feedback/master/CFO.owl#tools"/>
        <rdfs:comment>A comment related to the set of data and the type of data preferred to cover the theme in a training course</rdfs:comment>
        <rdfs:label>Dataset</rdfs:label>
    </owl:Class>
    


    <!-- https://raw.githubusercontent.com/GTPB/Training_Course_Feedback/master/CFO.owl#delivery -->

    <owl:Class rdf:about="https://raw.githubusercontent.com/GTPB/Training_Course_Feedback/master/CFO.owl#delivery">
        <rdfs:subClassOf rdf:resource="https://raw.githubusercontent.com/GTPB/Training_Course_Feedback/master/CFO.owl#tag_descriptor"/>
    </owl:Class>
    


    <!-- https://raw.githubusercontent.com/GTPB/Training_Course_Feedback/master/CFO.owl#depth -->

    <owl:Class rdf:about="https://raw.githubusercontent.com/GTPB/Training_Course_Feedback/master/CFO.owl#depth">
        <rdfs:subClassOf rdf:resource="https://raw.githubusercontent.com/GTPB/Training_Course_Feedback/master/CFO.owl#educational_content"/>
        <rdfs:comment>A comment related to the depth of the contents delivered in a training course</rdfs:comment>
        <rdfs:label>Depth</rdfs:label>
    </owl:Class>
    


    <!-- https://raw.githubusercontent.com/GTPB/Training_Course_Feedback/master/CFO.owl#description -->

    <owl:Class rdf:about="https://raw.githubusercontent.com/GTPB/Training_Course_Feedback/master/CFO.owl#description">
        <rdfs:subClassOf rdf:resource="https://raw.githubusercontent.com/GTPB/Training_Course_Feedback/master/CFO.owl#announcement"/>
        <rdfs:comment>A comment related to the information presented in the advertisement notice</rdfs:comment>
        <rdfs:label>Description</rdfs:label>
    </owl:Class>
    


    <!-- https://raw.githubusercontent.com/GTPB/Training_Course_Feedback/master/CFO.owl#directions -->

    <owl:Class rdf:about="https://raw.githubusercontent.com/GTPB/Training_Course_Feedback/master/CFO.owl#directions">
        <rdfs:subClassOf rdf:resource="https://raw.githubusercontent.com/GTPB/Training_Course_Feedback/master/CFO.owl#participant_support"/>
        <rdfs:comment>A comment related to the welcoming of the participant in the first day of a training course. It includes the provision of instructions to the training room.</rdfs:comment>
        <rdfs:label>Directions</rdfs:label>
    </owl:Class>
    


    <!-- https://raw.githubusercontent.com/GTPB/Training_Course_Feedback/master/CFO.owl#discussion -->

    <owl:Class rdf:about="https://raw.githubusercontent.com/GTPB/Training_Course_Feedback/master/CFO.owl#discussion">
        <rdfs:subClassOf rdf:resource="https://raw.githubusercontent.com/GTPB/Training_Course_Feedback/master/CFO.owl#activity"/>
        <rdfs:comment>A comment related to the discussion component in a training course</rdfs:comment>
        <rdfs:label>Discussion</rdfs:label>
    </owl:Class>
    


    <!-- https://raw.githubusercontent.com/GTPB/Training_Course_Feedback/master/CFO.owl#documentation -->

    <owl:Class rdf:about="https://raw.githubusercontent.com/GTPB/Training_Course_Feedback/master/CFO.owl#documentation">
        <rdfs:subClassOf rdf:resource="https://raw.githubusercontent.com/GTPB/Training_Course_Feedback/master/CFO.owl#application"/>
        <rdfs:comment>A comment related to the documentation needed for the accomplishment of the application process</rdfs:comment>
        <rdfs:label>Documentation</rdfs:label>
    </owl:Class>
    


    <!-- https://raw.githubusercontent.com/GTPB/Training_Course_Feedback/master/CFO.owl#duration -->

    <owl:Class rdf:about="https://raw.githubusercontent.com/GTPB/Training_Course_Feedback/master/CFO.owl#duration">
        <rdfs:subClassOf rdf:resource="https://raw.githubusercontent.com/GTPB/Training_Course_Feedback/master/CFO.owl#course_design_and_delivery"/>
        <rdfs:comment>A comment related to the total length of a training course</rdfs:comment>
        <rdfs:label>Duration</rdfs:label>
    </owl:Class>
    


    <!-- https://raw.githubusercontent.com/GTPB/Training_Course_Feedback/master/CFO.owl#dynamic -->

    <owl:Class rdf:about="https://raw.githubusercontent.com/GTPB/Training_Course_Feedback/master/CFO.owl#dynamic">
        <rdfs:subClassOf rdf:resource="https://raw.githubusercontent.com/GTPB/Training_Course_Feedback/master/CFO.owl#testimonial"/>
        <rdfs:comment>The course was dynamic</rdfs:comment>
        <rdfs:label>Dynamic</rdfs:label>
    </owl:Class>
    


    <!-- https://raw.githubusercontent.com/GTPB/Training_Course_Feedback/master/CFO.owl#educational_content -->

    <owl:Class rdf:about="https://raw.githubusercontent.com/GTPB/Training_Course_Feedback/master/CFO.owl#educational_content">
        <rdfs:subClassOf rdf:resource="https://raw.githubusercontent.com/GTPB/Training_Course_Feedback/master/CFO.owl#strategies"/>
        <rdfs:comment>A subject related to the educational content designed and delivered in a training course</rdfs:comment>
        <rdfs:label>Educational content</rdfs:label>
    </owl:Class>
    


    <!-- https://raw.githubusercontent.com/GTPB/Training_Course_Feedback/master/CFO.owl#efficacy -->

    <owl:Class rdf:about="https://raw.githubusercontent.com/GTPB/Training_Course_Feedback/master/CFO.owl#efficacy">
        <rdfs:subClassOf rdf:resource="https://raw.githubusercontent.com/GTPB/Training_Course_Feedback/master/CFO.owl#tag_descriptor"/>
    </owl:Class>
    


    <!-- https://raw.githubusercontent.com/GTPB/Training_Course_Feedback/master/CFO.owl#environment -->

    <owl:Class rdf:about="https://raw.githubusercontent.com/GTPB/Training_Course_Feedback/master/CFO.owl#environment">
        <rdfs:subClassOf rdf:resource="https://raw.githubusercontent.com/GTPB/Training_Course_Feedback/master/CFO.owl#course_design_and_delivery"/>
        <rdfs:comment>A comment related to the environment established in a training course</rdfs:comment>
        <rdfs:label>Environment</rdfs:label>
    </owl:Class>
    


    <!-- https://raw.githubusercontent.com/GTPB/Training_Course_Feedback/master/CFO.owl#equipment -->

    <owl:Class rdf:about="https://raw.githubusercontent.com/GTPB/Training_Course_Feedback/master/CFO.owl#equipment">
        <rdfs:subClassOf rdf:resource="https://raw.githubusercontent.com/GTPB/Training_Course_Feedback/master/CFO.owl#resources"/>
        <rdfs:comment>A comment related to the equipment and technology used to assist a training course</rdfs:comment>
        <rdfs:label>Equipment</rdfs:label>
    </owl:Class>
    


    <!-- https://raw.githubusercontent.com/GTPB/Training_Course_Feedback/master/CFO.owl#exam -->

    <owl:Class rdf:about="https://raw.githubusercontent.com/GTPB/Training_Course_Feedback/master/CFO.owl#exam">
        <rdfs:subClassOf rdf:resource="https://raw.githubusercontent.com/GTPB/Training_Course_Feedback/master/CFO.owl#sumative_assess"/>
    </owl:Class>
    


    <!-- https://raw.githubusercontent.com/GTPB/Training_Course_Feedback/master/CFO.owl#examples -->

    <owl:Class rdf:about="https://raw.githubusercontent.com/GTPB/Training_Course_Feedback/master/CFO.owl#examples">
        <rdfs:subClassOf rdf:resource="https://raw.githubusercontent.com/GTPB/Training_Course_Feedback/master/CFO.owl#content_type"/>
        <rdfs:comment>A comment related to the examples used to cover the theme in a training course</rdfs:comment>
        <rdfs:label>Examples</rdfs:label>
    </owl:Class>
    


    <!-- https://raw.githubusercontent.com/GTPB/Training_Course_Feedback/master/CFO.owl#exercises -->

    <owl:Class rdf:about="https://raw.githubusercontent.com/GTPB/Training_Course_Feedback/master/CFO.owl#exercises">
        <rdfs:subClassOf rdf:resource="https://raw.githubusercontent.com/GTPB/Training_Course_Feedback/master/CFO.owl#content_type"/>
        <rdfs:comment>A comment related to the exercises used to cover the theme in a training course</rdfs:comment>
        <rdfs:label>Exercises</rdfs:label>
    </owl:Class>
    


    <!-- https://raw.githubusercontent.com/GTPB/Training_Course_Feedback/master/CFO.owl#expectations -->

    <owl:Class rdf:about="https://raw.githubusercontent.com/GTPB/Training_Course_Feedback/master/CFO.owl#expectations">
        <rdfs:subClassOf rdf:resource="https://raw.githubusercontent.com/GTPB/Training_Course_Feedback/master/CFO.owl#pre_course"/>
        <rdfs:comment>A comment related to what the participant expects to learn in a training course</rdfs:comment>
        <rdfs:label>Expectations</rdfs:label>
    </owl:Class>
    


    <!-- https://raw.githubusercontent.com/GTPB/Training_Course_Feedback/master/CFO.owl#explanations -->

    <owl:Class rdf:about="https://raw.githubusercontent.com/GTPB/Training_Course_Feedback/master/CFO.owl#explanations">
        <rdfs:subClassOf rdf:resource="https://raw.githubusercontent.com/GTPB/Training_Course_Feedback/master/CFO.owl#content_type"/>
        <rdfs:comment>A comment related to the explanations provided in a training course</rdfs:comment>
        <rdfs:label>Explanations</rdfs:label>
    </owl:Class>
    


    <!-- https://raw.githubusercontent.com/GTPB/Training_Course_Feedback/master/CFO.owl#extra_organization -->

    <owl:Class rdf:about="https://raw.githubusercontent.com/GTPB/Training_Course_Feedback/master/CFO.owl#extra_organization">
        <rdfs:subClassOf rdf:resource="https://raw.githubusercontent.com/GTPB/Training_Course_Feedback/master/CFO.owl#course_assessment"/>
        <rdfs:comment>A subject related to the functioning of a training course out of the scope of the organization team</rdfs:comment>
        <rdfs:label>Extra-organization</rdfs:label>
    </owl:Class>
    


    <!-- https://raw.githubusercontent.com/GTPB/Training_Course_Feedback/master/CFO.owl#fee -->

    <owl:Class rdf:about="https://raw.githubusercontent.com/GTPB/Training_Course_Feedback/master/CFO.owl#fee">
        <rdfs:subClassOf rdf:resource="https://raw.githubusercontent.com/GTPB/Training_Course_Feedback/master/CFO.owl#organization_centred"/>
        <rdfs:comment>A comment related to the fee of the course</rdfs:comment>
        <rdfs:label>Fee</rdfs:label>
    </owl:Class>
    


    <!-- https://raw.githubusercontent.com/GTPB/Training_Course_Feedback/master/CFO.owl#flipped_class -->

    <owl:Class rdf:about="https://raw.githubusercontent.com/GTPB/Training_Course_Feedback/master/CFO.owl#flipped_class">
        <rdfs:subClassOf rdf:resource="https://raw.githubusercontent.com/GTPB/Training_Course_Feedback/master/CFO.owl#methods"/>
        <rdfs:comment>A comment related to the adoption of the flipped classroom model in a training course</rdfs:comment>
        <rdfs:label>Flipped class</rdfs:label>
    </owl:Class>
    


    <!-- https://raw.githubusercontent.com/GTPB/Training_Course_Feedback/master/CFO.owl#formal_assess -->

    <owl:Class rdf:about="https://raw.githubusercontent.com/GTPB/Training_Course_Feedback/master/CFO.owl#formal_assess">
        <rdfs:subClassOf rdf:resource="https://raw.githubusercontent.com/GTPB/Training_Course_Feedback/master/CFO.owl#formative_assess"/>
        <rdfs:comment>A comment related to the use of an assessment instrument in a formal modality in a training course (e.g. questionnaires, socrative, etc)</rdfs:comment>
        <rdfs:label>Formal assess</rdfs:label>
    </owl:Class>
    


    <!-- https://raw.githubusercontent.com/GTPB/Training_Course_Feedback/master/CFO.owl#format -->

    <owl:Class rdf:about="https://raw.githubusercontent.com/GTPB/Training_Course_Feedback/master/CFO.owl#format">
        <rdfs:subClassOf rdf:resource="https://raw.githubusercontent.com/GTPB/Training_Course_Feedback/master/CFO.owl#tag_descriptor"/>
    </owl:Class>
    


    <!-- https://raw.githubusercontent.com/GTPB/Training_Course_Feedback/master/CFO.owl#formative_assess -->

    <owl:Class rdf:about="https://raw.githubusercontent.com/GTPB/Training_Course_Feedback/master/CFO.owl#formative_assess">
        <rdfs:subClassOf rdf:resource="https://raw.githubusercontent.com/GTPB/Training_Course_Feedback/master/CFO.owl#assessment_instruments"/>
        <rdfs:comment>A subject related to the formative assessment of participant&apos;s learning progress in a training course</rdfs:comment>
        <rdfs:label>Formative assess</rdfs:label>
    </owl:Class>
    


    <!-- https://raw.githubusercontent.com/GTPB/Training_Course_Feedback/master/CFO.owl#frequency -->

    <owl:Class rdf:about="https://raw.githubusercontent.com/GTPB/Training_Course_Feedback/master/CFO.owl#frequency">
        <rdfs:subClassOf rdf:resource="https://raw.githubusercontent.com/GTPB/Training_Course_Feedback/master/CFO.owl#tag_descriptor"/>
    </owl:Class>
    


    <!-- https://raw.githubusercontent.com/GTPB/Training_Course_Feedback/master/CFO.owl#furniture -->

    <owl:Class rdf:about="https://raw.githubusercontent.com/GTPB/Training_Course_Feedback/master/CFO.owl#furniture">
        <rdfs:subClassOf rdf:resource="https://raw.githubusercontent.com/GTPB/Training_Course_Feedback/master/CFO.owl#training_room"/>
        <rdfs:comment>A comment related to the furniture of the training room where a training course takes place</rdfs:comment>
        <rdfs:label>Furniture</rdfs:label>
    </owl:Class>
    


    <!-- https://raw.githubusercontent.com/GTPB/Training_Course_Feedback/master/CFO.owl#future_course_theme -->

    <owl:Class rdf:about="https://raw.githubusercontent.com/GTPB/Training_Course_Feedback/master/CFO.owl#future_course_theme">
        <rdfs:subClassOf rdf:resource="https://raw.githubusercontent.com/GTPB/Training_Course_Feedback/master/CFO.owl#participant_course_feedback_subject"/>
        <rdfs:comment>Course theme about which the participant would be interested in learning in the near future</rdfs:comment>
        <rdfs:label>Future course theme</rdfs:label>
    </owl:Class>
    


    <!-- https://raw.githubusercontent.com/GTPB/Training_Course_Feedback/master/CFO.owl#games -->

    <owl:Class rdf:about="https://raw.githubusercontent.com/GTPB/Training_Course_Feedback/master/CFO.owl#games">
        <rdfs:subClassOf rdf:resource="https://raw.githubusercontent.com/GTPB/Training_Course_Feedback/master/CFO.owl#content_type"/>
        <rdfs:comment>A comment related to the games proposed in a training course to enhance the learning experience</rdfs:comment>
        <rdfs:label>Games</rdfs:label>
    </owl:Class>
    


    <!-- https://raw.githubusercontent.com/GTPB/Training_Course_Feedback/master/CFO.owl#global -->

    <owl:Class rdf:about="https://raw.githubusercontent.com/GTPB/Training_Course_Feedback/master/CFO.owl#global">
        <rdfs:subClassOf rdf:resource="https://raw.githubusercontent.com/GTPB/Training_Course_Feedback/master/CFO.owl#modality"/>
        <rdfs:comment>A comment related to the global type of instruction delivered in a training course (i.e. activities performed synchronously by all the instructor(s) and participant(s)</rdfs:comment>
        <rdfs:label>Global</rdfs:label>
    </owl:Class>
    


    <!-- https://raw.githubusercontent.com/GTPB/Training_Course_Feedback/master/CFO.owl#goals -->

    <owl:Class rdf:about="https://raw.githubusercontent.com/GTPB/Training_Course_Feedback/master/CFO.owl#goals">
        <rdfs:subClassOf rdf:resource="https://raw.githubusercontent.com/GTPB/Training_Course_Feedback/master/CFO.owl#course_design_and_delivery"/>
        <rdfs:comment>A comment related to the aim and goals intended in a training course</rdfs:comment>
        <rdfs:label>Goals</rdfs:label>
    </owl:Class>
    


    <!-- https://raw.githubusercontent.com/GTPB/Training_Course_Feedback/master/CFO.owl#group_criteria -->

    <owl:Class rdf:about="https://raw.githubusercontent.com/GTPB/Training_Course_Feedback/master/CFO.owl#group_criteria">
        <rdfs:subClassOf rdf:resource="https://raw.githubusercontent.com/GTPB/Training_Course_Feedback/master/CFO.owl#grouping"/>
        <rdfs:comment>A comment related to the criteria behind the choice of groups formed in behalf of a training course</rdfs:comment>
    </owl:Class>
    


    <!-- https://raw.githubusercontent.com/GTPB/Training_Course_Feedback/master/CFO.owl#group_size -->

    <owl:Class rdf:about="https://raw.githubusercontent.com/GTPB/Training_Course_Feedback/master/CFO.owl#group_size">
        <rdfs:subClassOf rdf:resource="https://raw.githubusercontent.com/GTPB/Training_Course_Feedback/master/CFO.owl#grouping"/>
        <rdfs:comment>A comment related to the number of participants of  the groups formed in behalf of a training course</rdfs:comment>
        <rdfs:label>Group size</rdfs:label>
    </owl:Class>
    


    <!-- https://raw.githubusercontent.com/GTPB/Training_Course_Feedback/master/CFO.owl#grouping -->

    <owl:Class rdf:about="https://raw.githubusercontent.com/GTPB/Training_Course_Feedback/master/CFO.owl#grouping">
        <rdfs:subClassOf rdf:resource="https://raw.githubusercontent.com/GTPB/Training_Course_Feedback/master/CFO.owl#methods"/>
        <rdfs:comment>A comment related to the adoption of the technique of grouping the participants in a training course</rdfs:comment>
        <rdfs:label>Grouping</rdfs:label>
    </owl:Class>
    


    <!-- https://raw.githubusercontent.com/GTPB/Training_Course_Feedback/master/CFO.owl#guidance -->

    <owl:Class rdf:about="https://raw.githubusercontent.com/GTPB/Training_Course_Feedback/master/CFO.owl#guidance">
        <rdfs:subClassOf rdf:resource="https://raw.githubusercontent.com/GTPB/Training_Course_Feedback/master/CFO.owl#implementation"/>
        <rdfs:comment>A comment related to the use of the guidance technique to provide instruction in a training course</rdfs:comment>
        <rdfs:label>Guidance</rdfs:label>
    </owl:Class>
    


    <!-- https://raw.githubusercontent.com/GTPB/Training_Course_Feedback/master/CFO.owl#guideline -->

    <owl:Class rdf:about="https://raw.githubusercontent.com/GTPB/Training_Course_Feedback/master/CFO.owl#guideline">
        <rdfs:subClassOf rdf:resource="https://raw.githubusercontent.com/GTPB/Training_Course_Feedback/master/CFO.owl#auxiliary"/>
        <rdfs:comment>A comment related to the use of explicit guidelines to support the assignments and the comprehension of the theme covered in a training course</rdfs:comment>
        <rdfs:label>Guideline</rdfs:label>
    </owl:Class>
    


    <!-- https://raw.githubusercontent.com/GTPB/Training_Course_Feedback/master/CFO.owl#handouts -->

    <owl:Class rdf:about="https://raw.githubusercontent.com/GTPB/Training_Course_Feedback/master/CFO.owl#handouts">
        <rdfs:subClassOf rdf:resource="https://raw.githubusercontent.com/GTPB/Training_Course_Feedback/master/CFO.owl#materials"/>
        <rdfs:comment>A comment related to the materials that are provided to the participants of a training course to support the learning experience in time</rdfs:comment>
        <rdfs:label>Handouts</rdfs:label>
    </owl:Class>
    


    <!-- https://raw.githubusercontent.com/GTPB/Training_Course_Feedback/master/CFO.owl#hands_on -->

    <owl:Class rdf:about="https://raw.githubusercontent.com/GTPB/Training_Course_Feedback/master/CFO.owl#hands_on">
        <rdfs:subClassOf rdf:resource="https://raw.githubusercontent.com/GTPB/Training_Course_Feedback/master/CFO.owl#methods"/>
        <rdfs:comment>A comment related to the adoption of the hands-on model in a training course</rdfs:comment>
        <rdfs:label>Hands-on</rdfs:label>
    </owl:Class>
    


    <!-- https://raw.githubusercontent.com/GTPB/Training_Course_Feedback/master/CFO.owl#housing_and_parking -->

    <owl:Class rdf:about="https://raw.githubusercontent.com/GTPB/Training_Course_Feedback/master/CFO.owl#housing_and_parking">
        <rdfs:subClassOf rdf:resource="https://raw.githubusercontent.com/GTPB/Training_Course_Feedback/master/CFO.owl#participant_support"/>
        <rdfs:comment>A comment related to the accommodations and parking options available for the participant of a training course</rdfs:comment>
        <rdfs:label>Housing and parking</rdfs:label>
    </owl:Class>
    


    <!-- https://raw.githubusercontent.com/GTPB/Training_Course_Feedback/master/CFO.owl#impact -->

    <owl:Class rdf:about="https://raw.githubusercontent.com/GTPB/Training_Course_Feedback/master/CFO.owl#impact">
        <rdfs:subClassOf rdf:resource="https://raw.githubusercontent.com/GTPB/Training_Course_Feedback/master/CFO.owl#post_course"/>
        <rdfs:comment>A comment related to the foreseeable impact of a training course in the participant&apos;s point of view</rdfs:comment>
        <rdfs:label>Impact</rdfs:label>
    </owl:Class>
    


    <!-- https://raw.githubusercontent.com/GTPB/Training_Course_Feedback/master/CFO.owl#implementation -->

    <owl:Class rdf:about="https://raw.githubusercontent.com/GTPB/Training_Course_Feedback/master/CFO.owl#implementation">
        <rdfs:subClassOf rdf:resource="https://raw.githubusercontent.com/GTPB/Training_Course_Feedback/master/CFO.owl#instructional_methodology"/>
        <rdfs:comment>A subject related to the implementation of the methods and techniques in a training course</rdfs:comment>
        <rdfs:label>Implementation</rdfs:label>
    </owl:Class>
    


    <!-- https://raw.githubusercontent.com/GTPB/Training_Course_Feedback/master/CFO.owl#informal_assess -->

    <owl:Class rdf:about="https://raw.githubusercontent.com/GTPB/Training_Course_Feedback/master/CFO.owl#informal_assess">
        <rdfs:subClassOf rdf:resource="https://raw.githubusercontent.com/GTPB/Training_Course_Feedback/master/CFO.owl#formative_assess"/>
        <rdfs:comment>A comment related to the use of an assessment instrument in an informal modality in a training course (e.g. raising hands, lamp system, coloured post-its, etc)</rdfs:comment>
        <rdfs:label>Informal assess</rdfs:label>
    </owl:Class>
    


    <!-- https://raw.githubusercontent.com/GTPB/Training_Course_Feedback/master/CFO.owl#informative -->

    <owl:Class rdf:about="https://raw.githubusercontent.com/GTPB/Training_Course_Feedback/master/CFO.owl#informative">
        <rdfs:subClassOf rdf:resource="https://raw.githubusercontent.com/GTPB/Training_Course_Feedback/master/CFO.owl#testimonial"/>
        <rdfs:comment>The course was informative, enlightening</rdfs:comment>
        <rdfs:label>Informative</rdfs:label>
    </owl:Class>
    


    <!-- https://raw.githubusercontent.com/GTPB/Training_Course_Feedback/master/CFO.owl#input_file -->

    <owl:Class rdf:about="https://raw.githubusercontent.com/GTPB/Training_Course_Feedback/master/CFO.owl#input_file">
        <rdfs:subClassOf rdf:resource="https://raw.githubusercontent.com/GTPB/Training_Course_Feedback/master/CFO.owl#data_file"/>
        <rdfs:comment>A comment related to the input files used in a training course</rdfs:comment>
        <rdfs:label>Input file</rdfs:label>
    </owl:Class>
    


    <!-- https://raw.githubusercontent.com/GTPB/Training_Course_Feedback/master/CFO.owl#insightful -->

    <owl:Class rdf:about="https://raw.githubusercontent.com/GTPB/Training_Course_Feedback/master/CFO.owl#insightful">
        <rdfs:subClassOf rdf:resource="https://raw.githubusercontent.com/GTPB/Training_Course_Feedback/master/CFO.owl#impact"/>
        <rdfs:comment>The course was insightful, granting a deep and true understanding of the theme/topics.</rdfs:comment>
        <rdfs:label>Insightful</rdfs:label>
    </owl:Class>
    


    <!-- https://raw.githubusercontent.com/GTPB/Training_Course_Feedback/master/CFO.owl#inspiring_follow_up -->

    <owl:Class rdf:about="https://raw.githubusercontent.com/GTPB/Training_Course_Feedback/master/CFO.owl#inspiring_follow_up">
        <rdfs:subClassOf rdf:resource="https://raw.githubusercontent.com/GTPB/Training_Course_Feedback/master/CFO.owl#impact"/>
        <rdfs:comment>The course was inspiring. The course was motivating to continue deepening the subject area or working in it.</rdfs:comment>
        <rdfs:label>Inspiring to follow-up</rdfs:label>
    </owl:Class>
    


    <!-- https://raw.githubusercontent.com/GTPB/Training_Course_Feedback/master/CFO.owl#instructional_instruments -->

    <owl:Class rdf:about="https://raw.githubusercontent.com/GTPB/Training_Course_Feedback/master/CFO.owl#instructional_instruments">
        <rdfs:subClassOf rdf:resource="https://raw.githubusercontent.com/GTPB/Training_Course_Feedback/master/CFO.owl#strategies"/>
        <rdfs:comment>A subject related to the instruments selected to facilitate the learning experience in a training course</rdfs:comment>
        <rdfs:label>Instructional instruments</rdfs:label>
    </owl:Class>
    


    <!-- https://raw.githubusercontent.com/GTPB/Training_Course_Feedback/master/CFO.owl#instructional_methodology -->

    <owl:Class rdf:about="https://raw.githubusercontent.com/GTPB/Training_Course_Feedback/master/CFO.owl#instructional_methodology">
        <rdfs:subClassOf rdf:resource="https://raw.githubusercontent.com/GTPB/Training_Course_Feedback/master/CFO.owl#strategies"/>
        <rdfs:comment>A subject related to the instruction and methods designed and applied in a training course</rdfs:comment>
        <rdfs:label>Instructional methodology</rdfs:label>
    </owl:Class>
    


    <!-- https://raw.githubusercontent.com/GTPB/Training_Course_Feedback/master/CFO.owl#instructors -->

    <owl:Class rdf:about="https://raw.githubusercontent.com/GTPB/Training_Course_Feedback/master/CFO.owl#instructors">
        <rdfs:subClassOf rdf:resource="https://raw.githubusercontent.com/GTPB/Training_Course_Feedback/master/CFO.owl#staff"/>
        <rdfs:comment>A comment related to the team responsible for the pedagogical aspects (i.e. instruction) in a training course</rdfs:comment>
        <rdfs:label>Instructors</rdfs:label>
    </owl:Class>
    


    <!-- https://raw.githubusercontent.com/GTPB/Training_Course_Feedback/master/CFO.owl#integrative -->

    <owl:Class rdf:about="https://raw.githubusercontent.com/GTPB/Training_Course_Feedback/master/CFO.owl#integrative">
        <rdfs:subClassOf rdf:resource="https://raw.githubusercontent.com/GTPB/Training_Course_Feedback/master/CFO.owl#testimonial"/>
        <rdfs:comment>The course was integrative</rdfs:comment>
        <rdfs:label>Integrative</rdfs:label>
    </owl:Class>
    


    <!-- https://raw.githubusercontent.com/GTPB/Training_Course_Feedback/master/CFO.owl#intense -->

    <owl:Class rdf:about="https://raw.githubusercontent.com/GTPB/Training_Course_Feedback/master/CFO.owl#intense">
        <rdfs:subClassOf rdf:resource="https://raw.githubusercontent.com/GTPB/Training_Course_Feedback/master/CFO.owl#testimonial"/>
        <rdfs:comment>The course was intense</rdfs:comment>
        <rdfs:label>Intense</rdfs:label>
    </owl:Class>
    


    <!-- https://raw.githubusercontent.com/GTPB/Training_Course_Feedback/master/CFO.owl#interaction -->

    <owl:Class rdf:about="https://raw.githubusercontent.com/GTPB/Training_Course_Feedback/master/CFO.owl#interaction">
        <rdfs:subClassOf rdf:resource="https://raw.githubusercontent.com/GTPB/Training_Course_Feedback/master/CFO.owl#instructional_methodology"/>
        <rdfs:comment>A subject related to the interaction type facilitated in a training course</rdfs:comment>
        <rdfs:label>Interaction</rdfs:label>
    </owl:Class>
    


    <!-- https://raw.githubusercontent.com/GTPB/Training_Course_Feedback/master/CFO.owl#interaction_content -->

    <owl:Class rdf:about="https://raw.githubusercontent.com/GTPB/Training_Course_Feedback/master/CFO.owl#interaction_content">
        <rdfs:subClassOf rdf:resource="https://raw.githubusercontent.com/GTPB/Training_Course_Feedback/master/CFO.owl#interaction"/>
        <rdfs:comment>A comment related to the interaction promoted with the content in a training course</rdfs:comment>
        <rdfs:label>Interaction with the content</rdfs:label>
    </owl:Class>
    


    <!-- https://raw.githubusercontent.com/GTPB/Training_Course_Feedback/master/CFO.owl#interaction_instructor -->

    <owl:Class rdf:about="https://raw.githubusercontent.com/GTPB/Training_Course_Feedback/master/CFO.owl#interaction_instructor">
        <rdfs:subClassOf rdf:resource="https://raw.githubusercontent.com/GTPB/Training_Course_Feedback/master/CFO.owl#interaction"/>
        <rdfs:comment>A comment related to the interaction facilitated between the instructor(s) and the participant(s) in a training course</rdfs:comment>
        <rdfs:label>Interaction with instructor</rdfs:label>
    </owl:Class>
    


    <!-- https://raw.githubusercontent.com/GTPB/Training_Course_Feedback/master/CFO.owl#interaction_peers -->

    <owl:Class rdf:about="https://raw.githubusercontent.com/GTPB/Training_Course_Feedback/master/CFO.owl#interaction_peers">
        <rdfs:subClassOf rdf:resource="https://raw.githubusercontent.com/GTPB/Training_Course_Feedback/master/CFO.owl#interaction"/>
        <rdfs:comment>A comment related to the interaction facilitated between the participants in a training course</rdfs:comment>
        <rdfs:label>Interaction with peers</rdfs:label>
    </owl:Class>
    


    <!-- https://raw.githubusercontent.com/GTPB/Training_Course_Feedback/master/CFO.owl#interactivity -->

    <owl:Class rdf:about="https://raw.githubusercontent.com/GTPB/Training_Course_Feedback/master/CFO.owl#interactivity">
        <rdfs:subClassOf rdf:resource="https://raw.githubusercontent.com/GTPB/Training_Course_Feedback/master/CFO.owl#tag_descriptor"/>
    </owl:Class>
    


    <!-- https://raw.githubusercontent.com/GTPB/Training_Course_Feedback/master/CFO.owl#interesting -->

    <owl:Class rdf:about="https://raw.githubusercontent.com/GTPB/Training_Course_Feedback/master/CFO.owl#interesting">
        <rdfs:subClassOf rdf:resource="https://raw.githubusercontent.com/GTPB/Training_Course_Feedback/master/CFO.owl#testimonial"/>
        <rdfs:comment>The course was interesting</rdfs:comment>
        <rdfs:label>Interesting</rdfs:label>
    </owl:Class>
    


    <!-- https://raw.githubusercontent.com/GTPB/Training_Course_Feedback/master/CFO.owl#introduction -->

    <owl:Class rdf:about="https://raw.githubusercontent.com/GTPB/Training_Course_Feedback/master/CFO.owl#introduction">
        <rdfs:subClassOf rdf:resource="https://raw.githubusercontent.com/GTPB/Training_Course_Feedback/master/CFO.owl#content_scheme"/>
        <rdfs:comment>A comment related to the introduction part of the topic in a training course</rdfs:comment>
        <rdfs:label>Introduction</rdfs:label>
    </owl:Class>
    


    <!-- https://raw.githubusercontent.com/GTPB/Training_Course_Feedback/master/CFO.owl#knowledge_improvement -->

    <owl:Class rdf:about="https://raw.githubusercontent.com/GTPB/Training_Course_Feedback/master/CFO.owl#knowledge_improvement">
        <rdfs:subClassOf rdf:resource="https://raw.githubusercontent.com/GTPB/Training_Course_Feedback/master/CFO.owl#self_assessment"/>
        <rdfs:comment>The participant believes to have improved in knowledge on the subject theme addressed in a training course</rdfs:comment>
        <rdfs:label>Knowledge improvement</rdfs:label>
    </owl:Class>
    


    <!-- https://raw.githubusercontent.com/GTPB/Training_Course_Feedback/master/CFO.owl#knowledge_type -->

    <owl:Class rdf:about="https://raw.githubusercontent.com/GTPB/Training_Course_Feedback/master/CFO.owl#knowledge_type">
        <rdfs:subClassOf rdf:resource="https://raw.githubusercontent.com/GTPB/Training_Course_Feedback/master/CFO.owl#future_course_theme"/>
        <rdfs:comment>The type of knowledge the participant is interested in learning about a subject theme in a future course</rdfs:comment>
        <rdfs:label>Knowledge type</rdfs:label>
    </owl:Class>
    


    <!-- https://raw.githubusercontent.com/GTPB/Training_Course_Feedback/master/CFO.owl#language_fluency -->

    <owl:Class rdf:about="https://raw.githubusercontent.com/GTPB/Training_Course_Feedback/master/CFO.owl#language_fluency">
        <rdfs:subClassOf rdf:resource="https://raw.githubusercontent.com/GTPB/Training_Course_Feedback/master/CFO.owl#instructors"/>
        <rdfs:comment>A comment related to the language fluency of the members of the team involved in a training course</rdfs:comment>
        <rdfs:label>Language fluency</rdfs:label>
    </owl:Class>
    


    <!-- https://raw.githubusercontent.com/GTPB/Training_Course_Feedback/master/CFO.owl#layout -->

    <owl:Class rdf:about="https://raw.githubusercontent.com/GTPB/Training_Course_Feedback/master/CFO.owl#layout">
        <rdfs:subClassOf rdf:resource="https://raw.githubusercontent.com/GTPB/Training_Course_Feedback/master/CFO.owl#tag_descriptor"/>
    </owl:Class>
    


    <!-- https://raw.githubusercontent.com/GTPB/Training_Course_Feedback/master/CFO.owl#lecture -->

    <owl:Class rdf:about="https://raw.githubusercontent.com/GTPB/Training_Course_Feedback/master/CFO.owl#lecture">
        <rdfs:subClassOf rdf:resource="https://raw.githubusercontent.com/GTPB/Training_Course_Feedback/master/CFO.owl#activity"/>
        <rdfs:comment>A comment related to the lecture component in a training course</rdfs:comment>
        <rdfs:label>Lecture</rdfs:label>
    </owl:Class>
    


    <!-- https://raw.githubusercontent.com/GTPB/Training_Course_Feedback/master/CFO.owl#lecturing -->

    <owl:Class rdf:about="https://raw.githubusercontent.com/GTPB/Training_Course_Feedback/master/CFO.owl#lecturing">
        <rdfs:subClassOf rdf:resource="https://raw.githubusercontent.com/GTPB/Training_Course_Feedback/master/CFO.owl#methods"/>
        <rdfs:comment>A comment related to the adoption of the lecturing model in a training course</rdfs:comment>
        <rdfs:label>Lecturing</rdfs:label>
    </owl:Class>
    


    <!-- https://raw.githubusercontent.com/GTPB/Training_Course_Feedback/master/CFO.owl#level -->

    <owl:Class rdf:about="https://raw.githubusercontent.com/GTPB/Training_Course_Feedback/master/CFO.owl#level">
        <rdfs:subClassOf rdf:resource="https://raw.githubusercontent.com/GTPB/Training_Course_Feedback/master/CFO.owl#educational_content"/>
        <rdfs:comment>A comment related to the level of the contents delivered in the training course</rdfs:comment>
        <rdfs:label>Level</rdfs:label>
    </owl:Class>
    


    <!-- https://raw.githubusercontent.com/GTPB/Training_Course_Feedback/master/CFO.owl#lighting -->

    <owl:Class rdf:about="https://raw.githubusercontent.com/GTPB/Training_Course_Feedback/master/CFO.owl#lighting">
        <rdfs:subClassOf rdf:resource="https://raw.githubusercontent.com/GTPB/Training_Course_Feedback/master/CFO.owl#climate"/>
        <rdfs:comment>A comment related to the light quality of the training room where a training course takes place</rdfs:comment>
        <rdfs:label>Lighting</rdfs:label>
    </owl:Class>
    


    <!-- https://raw.githubusercontent.com/GTPB/Training_Course_Feedback/master/CFO.owl#live_scripting -->

    <owl:Class rdf:about="https://raw.githubusercontent.com/GTPB/Training_Course_Feedback/master/CFO.owl#live_scripting">
        <rdfs:subClassOf rdf:resource="https://raw.githubusercontent.com/GTPB/Training_Course_Feedback/master/CFO.owl#implementation"/>
        <rdfs:comment>A comment related to the use of the live scripting technique to provide instruction in a training course</rdfs:comment>
        <rdfs:label>Live scripting</rdfs:label>
    </owl:Class>
    


    <!-- https://raw.githubusercontent.com/GTPB/Training_Course_Feedback/master/CFO.owl#load -->

    <owl:Class rdf:about="https://raw.githubusercontent.com/GTPB/Training_Course_Feedback/master/CFO.owl#load">
        <rdfs:subClassOf rdf:resource="https://raw.githubusercontent.com/GTPB/Training_Course_Feedback/master/CFO.owl#educational_content"/>
        <rdfs:comment>A comment related to the content loading in a training course</rdfs:comment>
        <rdfs:label>Load</rdfs:label>
    </owl:Class>
    


    <!-- https://raw.githubusercontent.com/GTPB/Training_Course_Feedback/master/CFO.owl#location -->

    <owl:Class rdf:about="https://raw.githubusercontent.com/GTPB/Training_Course_Feedback/master/CFO.owl#location">
        <rdfs:subClassOf rdf:resource="https://raw.githubusercontent.com/GTPB/Training_Course_Feedback/master/CFO.owl#course_logistics"/>
        <rdfs:comment>A comment related to a training course site (including the location of the coffee-breaks)</rdfs:comment>
        <rdfs:label>Location</rdfs:label>
    </owl:Class>
    


    <!-- https://raw.githubusercontent.com/GTPB/Training_Course_Feedback/master/CFO.owl#materials -->

    <owl:Class rdf:about="https://raw.githubusercontent.com/GTPB/Training_Course_Feedback/master/CFO.owl#materials">
        <rdfs:subClassOf rdf:resource="https://raw.githubusercontent.com/GTPB/Training_Course_Feedback/master/CFO.owl#course_design_and_delivery"/>
        <rdfs:comment>A subject related to the materials designed and presented in a training course</rdfs:comment>
        <rdfs:label>Materials</rdfs:label>
    </owl:Class>
    


    <!-- https://raw.githubusercontent.com/GTPB/Training_Course_Feedback/master/CFO.owl#methods -->

    <owl:Class rdf:about="https://raw.githubusercontent.com/GTPB/Training_Course_Feedback/master/CFO.owl#methods">
        <rdfs:subClassOf rdf:resource="https://raw.githubusercontent.com/GTPB/Training_Course_Feedback/master/CFO.owl#instructional_methodology"/>
        <rdfs:comment>A subject related to the method(s) and technique(s) adopted in a training course</rdfs:comment>
        <rdfs:label>Methods</rdfs:label>
    </owl:Class>
    


    <!-- https://raw.githubusercontent.com/GTPB/Training_Course_Feedback/master/CFO.owl#modality -->

    <owl:Class rdf:about="https://raw.githubusercontent.com/GTPB/Training_Course_Feedback/master/CFO.owl#modality">
        <rdfs:subClassOf rdf:resource="https://raw.githubusercontent.com/GTPB/Training_Course_Feedback/master/CFO.owl#instructional_methodology"/>
        <rdfs:comment>A subject related to the modality of instruction in a training course</rdfs:comment>
        <rdfs:label>Modality</rdfs:label>
    </owl:Class>
    


    <!-- https://raw.githubusercontent.com/GTPB/Training_Course_Feedback/master/CFO.owl#motivation -->

    <owl:Class rdf:about="https://raw.githubusercontent.com/GTPB/Training_Course_Feedback/master/CFO.owl#motivation">
        <rdfs:subClassOf rdf:resource="https://raw.githubusercontent.com/GTPB/Training_Course_Feedback/master/CFO.owl#contextualization"/>
        <rdfs:comment>A comment about the reasons that led the participant to attend a training course</rdfs:comment>
        <rdfs:label>Motivation</rdfs:label>
    </owl:Class>
    


    <!-- https://raw.githubusercontent.com/GTPB/Training_Course_Feedback/master/CFO.owl#navigability -->

    <owl:Class rdf:about="https://raw.githubusercontent.com/GTPB/Training_Course_Feedback/master/CFO.owl#navigability">
        <rdfs:subClassOf rdf:resource="https://raw.githubusercontent.com/GTPB/Training_Course_Feedback/master/CFO.owl#tag_descriptor"/>
    </owl:Class>
    


    <!-- https://raw.githubusercontent.com/GTPB/Training_Course_Feedback/master/CFO.owl#need_more_study -->

    <owl:Class rdf:about="https://raw.githubusercontent.com/GTPB/Training_Course_Feedback/master/CFO.owl#need_more_study">
        <rdfs:subClassOf rdf:resource="https://raw.githubusercontent.com/GTPB/Training_Course_Feedback/master/CFO.owl#self_assessment"/>
        <rdfs:comment>The participant believes that needs more study to get confidence in the subject theme addressed in a training course</rdfs:comment>
        <rdfs:label>Need more study</rdfs:label>
    </owl:Class>
    


    <!-- https://raw.githubusercontent.com/GTPB/Training_Course_Feedback/master/CFO.owl#negative -->

    <owl:Class rdf:about="https://raw.githubusercontent.com/GTPB/Training_Course_Feedback/master/CFO.owl#negative">
        <rdfs:subClassOf rdf:resource="https://raw.githubusercontent.com/GTPB/Training_Course_Feedback/master/CFO.owl#tag_qualifier"/>
    </owl:Class>
    


    <!-- https://raw.githubusercontent.com/GTPB/Training_Course_Feedback/master/CFO.owl#network_connection -->

    <owl:Class rdf:about="https://raw.githubusercontent.com/GTPB/Training_Course_Feedback/master/CFO.owl#network_connection">
        <rdfs:subClassOf rdf:resource="https://raw.githubusercontent.com/GTPB/Training_Course_Feedback/master/CFO.owl#equipment"/>
        <rdfs:comment>A comment related to the network connection used in a training course</rdfs:comment>
        <rdfs:label>Network_connection</rdfs:label>
    </owl:Class>
    


    <!-- https://raw.githubusercontent.com/GTPB/Training_Course_Feedback/master/CFO.owl#network_opportunity -->

    <owl:Class rdf:about="https://raw.githubusercontent.com/GTPB/Training_Course_Feedback/master/CFO.owl#network_opportunity">
        <rdfs:subClassOf rdf:resource="https://raw.githubusercontent.com/GTPB/Training_Course_Feedback/master/CFO.owl#impact"/>
        <rdfs:comment>The course consisted in an opportunity to network</rdfs:comment>
        <rdfs:label>Network opportunity</rdfs:label>
    </owl:Class>
    


    <!-- https://raw.githubusercontent.com/GTPB/Training_Course_Feedback/master/CFO.owl#noise -->

    <owl:Class rdf:about="https://raw.githubusercontent.com/GTPB/Training_Course_Feedback/master/CFO.owl#noise">
        <rdfs:subClassOf rdf:resource="https://raw.githubusercontent.com/GTPB/Training_Course_Feedback/master/CFO.owl#climate"/>
        <rdfs:comment>A comment related to the soundproof system and the noise of the training room where a training course takes place</rdfs:comment>
        <rdfs:label>Noise</rdfs:label>
    </owl:Class>
    


    <!-- https://raw.githubusercontent.com/GTPB/Training_Course_Feedback/master/CFO.owl#none -->

    <owl:Class rdf:about="https://raw.githubusercontent.com/GTPB/Training_Course_Feedback/master/CFO.owl#none">
        <rdfs:subClassOf rdf:resource="https://raw.githubusercontent.com/GTPB/Training_Course_Feedback/master/CFO.owl#tag_qualifier"/>
    </owl:Class>
    


    <!-- https://raw.githubusercontent.com/GTPB/Training_Course_Feedback/master/CFO.owl#number -->

    <owl:Class rdf:about="https://raw.githubusercontent.com/GTPB/Training_Course_Feedback/master/CFO.owl#number">
        <rdfs:subClassOf rdf:resource="https://raw.githubusercontent.com/GTPB/Training_Course_Feedback/master/CFO.owl#instructors"/>
        <rdfs:comment>A comment related to the number that comprise the team involved in a training course</rdfs:comment>
        <rdfs:label>Number</rdfs:label>
    </owl:Class>
    


    <!-- https://raw.githubusercontent.com/GTPB/Training_Course_Feedback/master/CFO.owl#object -->

    <owl:Class rdf:about="https://raw.githubusercontent.com/GTPB/Training_Course_Feedback/master/CFO.owl#object">
        <rdfs:subClassOf rdf:resource="https://raw.githubusercontent.com/GTPB/Training_Course_Feedback/master/CFO.owl#educational_content"/>
        <rdfs:comment>A comment related to the organism or system selected to illustrate the theme covered in a training course</rdfs:comment>
        <rdfs:label>Object</rdfs:label>
    </owl:Class>
    


    <!-- https://raw.githubusercontent.com/GTPB/Training_Course_Feedback/master/CFO.owl#office_supplies -->

    <owl:Class rdf:about="https://raw.githubusercontent.com/GTPB/Training_Course_Feedback/master/CFO.owl#office_supplies">
        <rdfs:subClassOf rdf:resource="https://raw.githubusercontent.com/GTPB/Training_Course_Feedback/master/CFO.owl#participant_support"/>
        <rdfs:comment>A comment related to the provision of office material (e.g. pens, notepads, etc) in a training course</rdfs:comment>
        <rdfs:label>Office supplies</rdfs:label>
    </owl:Class>
    


    <!-- https://raw.githubusercontent.com/GTPB/Training_Course_Feedback/master/CFO.owl#open_minded -->

    <owl:Class rdf:about="https://raw.githubusercontent.com/GTPB/Training_Course_Feedback/master/CFO.owl#open_minded">
        <rdfs:subClassOf rdf:resource="https://raw.githubusercontent.com/GTPB/Training_Course_Feedback/master/CFO.owl#impact"/>
        <rdfs:comment>The course opened new horizonts</rdfs:comment>
        <rdfs:label>Open-minded</rdfs:label>
    </owl:Class>
    


    <!-- https://raw.githubusercontent.com/GTPB/Training_Course_Feedback/master/CFO.owl#operating_system -->

    <owl:Class rdf:about="https://raw.githubusercontent.com/GTPB/Training_Course_Feedback/master/CFO.owl#operating_system">
        <rdfs:subClassOf rdf:resource="https://raw.githubusercontent.com/GTPB/Training_Course_Feedback/master/CFO.owl#equipment"/>
        <rdfs:comment>A comment related to the operating system used to run a training course</rdfs:comment>
        <rdfs:label>Operating_system</rdfs:label>
    </owl:Class>
    


    <!-- https://raw.githubusercontent.com/GTPB/Training_Course_Feedback/master/CFO.owl#operationality -->

    <owl:Class rdf:about="https://raw.githubusercontent.com/GTPB/Training_Course_Feedback/master/CFO.owl#operationality">
        <rdfs:subClassOf rdf:resource="https://raw.githubusercontent.com/GTPB/Training_Course_Feedback/master/CFO.owl#tag_descriptor"/>
    </owl:Class>
    


    <!-- https://raw.githubusercontent.com/GTPB/Training_Course_Feedback/master/CFO.owl#organization_centred -->

    <owl:Class rdf:about="https://raw.githubusercontent.com/GTPB/Training_Course_Feedback/master/CFO.owl#organization_centred">
        <rdfs:subClassOf rdf:resource="https://raw.githubusercontent.com/GTPB/Training_Course_Feedback/master/CFO.owl#course_assessment"/>
        <rdfs:comment>A subject related to the organization of a training course in which the organization team is directly involved</rdfs:comment>
        <rdfs:label>Organization centred</rdfs:label>
    </owl:Class>
    


    <!-- https://raw.githubusercontent.com/GTPB/Training_Course_Feedback/master/CFO.owl#organizers -->

    <owl:Class rdf:about="https://raw.githubusercontent.com/GTPB/Training_Course_Feedback/master/CFO.owl#organizers">
        <rdfs:subClassOf rdf:resource="https://raw.githubusercontent.com/GTPB/Training_Course_Feedback/master/CFO.owl#staff"/>
        <rdfs:comment>A comment related to the team responsible for the organizational aspects of a training course</rdfs:comment>
        <rdfs:label>Organizers</rdfs:label>
    </owl:Class>
    


    <!-- https://raw.githubusercontent.com/GTPB/Training_Course_Feedback/master/CFO.owl#output_file -->

    <owl:Class rdf:about="https://raw.githubusercontent.com/GTPB/Training_Course_Feedback/master/CFO.owl#output_file">
        <rdfs:subClassOf rdf:resource="https://raw.githubusercontent.com/GTPB/Training_Course_Feedback/master/CFO.owl#data_file"/>
        <rdfs:comment>A comment related to the output files and results produced in a training course</rdfs:comment>
        <rdfs:label>Output file</rdfs:label>
    </owl:Class>
    


    <!-- https://raw.githubusercontent.com/GTPB/Training_Course_Feedback/master/CFO.owl#own_data -->

    <owl:Class rdf:about="https://raw.githubusercontent.com/GTPB/Training_Course_Feedback/master/CFO.owl#own_data">
        <rdfs:subClassOf rdf:resource="https://raw.githubusercontent.com/GTPB/Training_Course_Feedback/master/CFO.owl#dataset"/>
        <rdfs:comment>A comment related to the use of participants own data to cover the theme in training course</rdfs:comment>
        <rdfs:label>Own data</rdfs:label>
    </owl:Class>
    


    <!-- https://raw.githubusercontent.com/GTPB/Training_Course_Feedback/master/CFO.owl#pace -->

    <owl:Class rdf:about="https://raw.githubusercontent.com/GTPB/Training_Course_Feedback/master/CFO.owl#pace">
        <rdfs:subClassOf rdf:resource="https://raw.githubusercontent.com/GTPB/Training_Course_Feedback/master/CFO.owl#course_design_and_delivery"/>
        <rdfs:comment>A comment related to the pace imposed in a training course</rdfs:comment>
        <rdfs:label>Pace</rdfs:label>
    </owl:Class>
    


    <!-- https://raw.githubusercontent.com/GTPB/Training_Course_Feedback/master/CFO.owl#participant_centred -->

    <owl:Class rdf:about="https://raw.githubusercontent.com/GTPB/Training_Course_Feedback/master/CFO.owl#participant_centred">
        <rdfs:subClassOf rdf:resource="https://raw.githubusercontent.com/GTPB/Training_Course_Feedback/master/CFO.owl#course_assessment"/>
        <rdfs:comment>A subject related to the participant attendance and experience in a training course</rdfs:comment>
        <rdfs:label>Participant centred</rdfs:label>
    </owl:Class>
    


    <!-- https://raw.githubusercontent.com/GTPB/Training_Course_Feedback/master/CFO.owl#participant_course_feedback_subject -->

    <owl:Class rdf:about="https://raw.githubusercontent.com/GTPB/Training_Course_Feedback/master/CFO.owl#participant_course_feedback_subject">
        <rdfs:comment xml:lang="en">A subject related to a training course about which the participant provides feedback</rdfs:comment>
        <rdfs:label xml:lang="en">Participant course feedback subject</rdfs:label>
    </owl:Class>
    


    <!-- https://raw.githubusercontent.com/GTPB/Training_Course_Feedback/master/CFO.owl#participant_support -->

    <owl:Class rdf:about="https://raw.githubusercontent.com/GTPB/Training_Course_Feedback/master/CFO.owl#participant_support">
        <rdfs:subClassOf rdf:resource="https://raw.githubusercontent.com/GTPB/Training_Course_Feedback/master/CFO.owl#course_logistics"/>
        <rdfs:comment>A subject related to the support provided to the participant enrolled in a training course</rdfs:comment>
        <rdfs:label>Participant support</rdfs:label>
    </owl:Class>
    


    <!-- https://raw.githubusercontent.com/GTPB/Training_Course_Feedback/master/CFO.owl#payment -->

    <owl:Class rdf:about="https://raw.githubusercontent.com/GTPB/Training_Course_Feedback/master/CFO.owl#payment">
        <rdfs:subClassOf rdf:resource="https://raw.githubusercontent.com/GTPB/Training_Course_Feedback/master/CFO.owl#registration"/>
        <rdfs:comment>A comment related to the payment process and procedures of a training course</rdfs:comment>
        <rdfs:label>Payment</rdfs:label>
    </owl:Class>
    


    <!-- https://raw.githubusercontent.com/GTPB/Training_Course_Feedback/master/CFO.owl#personalized -->

    <owl:Class rdf:about="https://raw.githubusercontent.com/GTPB/Training_Course_Feedback/master/CFO.owl#personalized">
        <rdfs:subClassOf rdf:resource="https://raw.githubusercontent.com/GTPB/Training_Course_Feedback/master/CFO.owl#modality"/>
        <rdfs:comment>A comment related to the personalized type of instruction delivered in a training course (i.e. activities directed to the participant&apos;s particular interests)</rdfs:comment>
        <rdfs:label>Personalized</rdfs:label>
    </owl:Class>
    


    <!-- https://raw.githubusercontent.com/GTPB/Training_Course_Feedback/master/CFO.owl#plenty -->

    <owl:Class rdf:about="https://raw.githubusercontent.com/GTPB/Training_Course_Feedback/master/CFO.owl#plenty">
        <rdfs:subClassOf rdf:resource="https://raw.githubusercontent.com/GTPB/Training_Course_Feedback/master/CFO.owl#tag_qualifier"/>
    </owl:Class>
    


    <!-- https://raw.githubusercontent.com/GTPB/Training_Course_Feedback/master/CFO.owl#positive -->

    <owl:Class rdf:about="https://raw.githubusercontent.com/GTPB/Training_Course_Feedback/master/CFO.owl#positive">
        <rdfs:subClassOf rdf:resource="https://raw.githubusercontent.com/GTPB/Training_Course_Feedback/master/CFO.owl#tag_qualifier"/>
    </owl:Class>
    


    <!-- https://raw.githubusercontent.com/GTPB/Training_Course_Feedback/master/CFO.owl#post_course -->

    <owl:Class rdf:about="https://raw.githubusercontent.com/GTPB/Training_Course_Feedback/master/CFO.owl#post_course">
        <rdfs:subClassOf rdf:resource="https://raw.githubusercontent.com/GTPB/Training_Course_Feedback/master/CFO.owl#participant_centred"/>
        <rdfs:comment>A subject related to the feedback shared by a participant after attending a training course</rdfs:comment>
        <rdfs:label>Post-course</rdfs:label>
    </owl:Class>
    


    <!-- https://raw.githubusercontent.com/GTPB/Training_Course_Feedback/master/CFO.owl#practice -->

    <owl:Class rdf:about="https://raw.githubusercontent.com/GTPB/Training_Course_Feedback/master/CFO.owl#practice">
        <rdfs:subClassOf rdf:resource="https://raw.githubusercontent.com/GTPB/Training_Course_Feedback/master/CFO.owl#activity"/>
        <rdfs:comment>A comment related to the practical component in a training course</rdfs:comment>
        <rdfs:label>Practice</rdfs:label>
    </owl:Class>
    


    <!-- https://raw.githubusercontent.com/GTPB/Training_Course_Feedback/master/CFO.owl#pre_course -->

    <owl:Class rdf:about="https://raw.githubusercontent.com/GTPB/Training_Course_Feedback/master/CFO.owl#pre_course">
        <rdfs:subClassOf rdf:resource="https://raw.githubusercontent.com/GTPB/Training_Course_Feedback/master/CFO.owl#participant_centred"/>
        <rdfs:comment>A subject related to an aspect concerning the experience of a participant before attending a training course</rdfs:comment>
        <rdfs:label>Pre-course</rdfs:label>
    </owl:Class>
    


    <!-- https://raw.githubusercontent.com/GTPB/Training_Course_Feedback/master/CFO.owl#prerequisites -->

    <owl:Class rdf:about="https://raw.githubusercontent.com/GTPB/Training_Course_Feedback/master/CFO.owl#prerequisites">
        <rdfs:subClassOf rdf:resource="https://raw.githubusercontent.com/GTPB/Training_Course_Feedback/master/CFO.owl#course_design_and_delivery"/>
        <rdfs:comment>A comment related to the prerequesites required to a gratified experience in a training course</rdfs:comment>
        <rdfs:label>Prerequisites</rdfs:label>
    </owl:Class>
    


    <!-- https://raw.githubusercontent.com/GTPB/Training_Course_Feedback/master/CFO.owl#presentations -->

    <owl:Class rdf:about="https://raw.githubusercontent.com/GTPB/Training_Course_Feedback/master/CFO.owl#presentations">
        <rdfs:subClassOf rdf:resource="https://raw.githubusercontent.com/GTPB/Training_Course_Feedback/master/CFO.owl#materials"/>
        <rdfs:comment>A comment related to the slide presentations displayed in a training course</rdfs:comment>
        <rdfs:label>Presentations</rdfs:label>
    </owl:Class>
    


    <!-- https://raw.githubusercontent.com/GTPB/Training_Course_Feedback/master/CFO.owl#previous_course -->

    <owl:Class rdf:about="https://raw.githubusercontent.com/GTPB/Training_Course_Feedback/master/CFO.owl#previous_course">
        <rdfs:subClassOf rdf:resource="https://raw.githubusercontent.com/GTPB/Training_Course_Feedback/master/CFO.owl#participant_support"/>
        <rdfs:comment>A comment related to the organization of a thematic course prior to a training course</rdfs:comment>
        <rdfs:label>Previous_course</rdfs:label>
    </owl:Class>
    


    <!-- https://raw.githubusercontent.com/GTPB/Training_Course_Feedback/master/CFO.owl#previous_knowledge -->

    <owl:Class rdf:about="https://raw.githubusercontent.com/GTPB/Training_Course_Feedback/master/CFO.owl#previous_knowledge">
        <rdfs:subClassOf rdf:resource="https://raw.githubusercontent.com/GTPB/Training_Course_Feedback/master/CFO.owl#background"/>
        <rdfs:comment>A comment related to the participant&apos;s previous knowledge in the subject covered in a training course</rdfs:comment>
        <rdfs:label>Previous knowledge</rdfs:label>
    </owl:Class>
    


    <!-- https://raw.githubusercontent.com/GTPB/Training_Course_Feedback/master/CFO.owl#previous_skill -->

    <owl:Class rdf:about="https://raw.githubusercontent.com/GTPB/Training_Course_Feedback/master/CFO.owl#previous_skill">
        <rdfs:subClassOf rdf:resource="https://raw.githubusercontent.com/GTPB/Training_Course_Feedback/master/CFO.owl#background"/>
        <rdfs:comment>A comment related to the participant&apos; skills in the tools used in a training course</rdfs:comment>
        <rdfs:label>Previous skill</rdfs:label>
    </owl:Class>
    


    <!-- https://raw.githubusercontent.com/GTPB/Training_Course_Feedback/master/CFO.owl#proficiency -->

    <owl:Class rdf:about="https://raw.githubusercontent.com/GTPB/Training_Course_Feedback/master/CFO.owl#proficiency">
        <rdfs:subClassOf rdf:resource="https://raw.githubusercontent.com/GTPB/Training_Course_Feedback/master/CFO.owl#instructors"/>
        <rdfs:subClassOf rdf:resource="https://raw.githubusercontent.com/GTPB/Training_Course_Feedback/master/CFO.owl#tag_descriptor"/>
        <rdfs:comment>A comment related to the proficiency of the pedagogical team perceived by the participant of a training course</rdfs:comment>
        <rdfs:label>Proficiency</rdfs:label>
    </owl:Class>
    


    <!-- https://raw.githubusercontent.com/GTPB/Training_Course_Feedback/master/CFO.owl#profitable -->

    <owl:Class rdf:about="https://raw.githubusercontent.com/GTPB/Training_Course_Feedback/master/CFO.owl#profitable">
        <rdfs:subClassOf rdf:resource="https://raw.githubusercontent.com/GTPB/Training_Course_Feedback/master/CFO.owl#impact"/>
        <rdfs:comment>The course was beneficial, although not immediately useful for the current interests (e.g. as an opportunity to learn interesting topics and subjects)</rdfs:comment>
        <rdfs:label>Profitable</rdfs:label>
    </owl:Class>
    


    <!-- https://raw.githubusercontent.com/GTPB/Training_Course_Feedback/master/CFO.owl#projector -->

    <owl:Class rdf:about="https://raw.githubusercontent.com/GTPB/Training_Course_Feedback/master/CFO.owl#projector">
        <rdfs:subClassOf rdf:resource="https://raw.githubusercontent.com/GTPB/Training_Course_Feedback/master/CFO.owl#equipment"/>
        <rdfs:comment>A comment related to the projector system used in a training course</rdfs:comment>
        <rdfs:label>Projector</rdfs:label>
    </owl:Class>
    


    <!-- https://raw.githubusercontent.com/GTPB/Training_Course_Feedback/master/CFO.owl#publicity -->

    <owl:Class rdf:about="https://raw.githubusercontent.com/GTPB/Training_Course_Feedback/master/CFO.owl#publicity">
        <rdfs:subClassOf rdf:resource="https://raw.githubusercontent.com/GTPB/Training_Course_Feedback/master/CFO.owl#announcement"/>
        <rdfs:comment>A comment related to the advertising strategy of a training course</rdfs:comment>
        <rdfs:label>Publicity</rdfs:label>
    </owl:Class>
    


    <!-- https://raw.githubusercontent.com/GTPB/Training_Course_Feedback/master/CFO.owl#publicity_source -->

    <owl:Class rdf:about="https://raw.githubusercontent.com/GTPB/Training_Course_Feedback/master/CFO.owl#publicity_source">
        <rdfs:subClassOf rdf:resource="https://raw.githubusercontent.com/GTPB/Training_Course_Feedback/master/CFO.owl#participant_course_feedback_subject"/>
        <rdfs:comment xml:lang="en">Source where the participant learned about the course</rdfs:comment>
        <rdfs:label xml:lang="en">Publicity source</rdfs:label>
    </owl:Class>
    


    <!-- https://raw.githubusercontent.com/GTPB/Training_Course_Feedback/master/CFO.owl#punctuality -->

    <owl:Class rdf:about="https://raw.githubusercontent.com/GTPB/Training_Course_Feedback/master/CFO.owl#punctuality">
        <rdfs:subClassOf rdf:resource="https://raw.githubusercontent.com/GTPB/Training_Course_Feedback/master/CFO.owl#tag_descriptor"/>
        <rdfs:subClassOf rdf:resource="https://raw.githubusercontent.com/GTPB/Training_Course_Feedback/master/CFO.owl#timetable"/>
        <rdfs:comment>A comment related to the accuracy of the timing planned in the timetable in a training course</rdfs:comment>
        <rdfs:label>Punctuality</rdfs:label>
    </owl:Class>
    


    <!-- https://raw.githubusercontent.com/GTPB/Training_Course_Feedback/master/CFO.owl#quantity -->

    <owl:Class rdf:about="https://raw.githubusercontent.com/GTPB/Training_Course_Feedback/master/CFO.owl#quantity">
        <rdfs:subClassOf rdf:resource="https://raw.githubusercontent.com/GTPB/Training_Course_Feedback/master/CFO.owl#tag_descriptor"/>
    </owl:Class>
    


    <!-- https://raw.githubusercontent.com/GTPB/Training_Course_Feedback/master/CFO.owl#raw_data -->

    <owl:Class rdf:about="https://raw.githubusercontent.com/GTPB/Training_Course_Feedback/master/CFO.owl#raw_data">
        <rdfs:subClassOf rdf:resource="https://raw.githubusercontent.com/GTPB/Training_Course_Feedback/master/CFO.owl#dataset"/>
        <rdfs:comment>A comment related to the use of raw data to cover the theme in training course</rdfs:comment>
        <rdfs:label>Raw data</rdfs:label>
    </owl:Class>
    


    <!-- https://raw.githubusercontent.com/GTPB/Training_Course_Feedback/master/CFO.owl#real_data -->

    <owl:Class rdf:about="https://raw.githubusercontent.com/GTPB/Training_Course_Feedback/master/CFO.owl#real_data">
        <rdfs:subClassOf rdf:resource="https://raw.githubusercontent.com/GTPB/Training_Course_Feedback/master/CFO.owl#dataset"/>
        <rdfs:comment>A comment related to the use of real-life data to cover the theme in training course</rdfs:comment>
        <rdfs:label>Real data</rdfs:label>
    </owl:Class>
    


    <!-- https://raw.githubusercontent.com/GTPB/Training_Course_Feedback/master/CFO.owl#receipt -->

    <owl:Class rdf:about="https://raw.githubusercontent.com/GTPB/Training_Course_Feedback/master/CFO.owl#receipt">
        <rdfs:subClassOf rdf:resource="https://raw.githubusercontent.com/GTPB/Training_Course_Feedback/master/CFO.owl#application"/>
        <rdfs:comment>A comment related to the acknowledgement of delivery communication to the participant of a training course.</rdfs:comment>
        <rdfs:label>Receipt</rdfs:label>
    </owl:Class>
    


    <!-- https://raw.githubusercontent.com/GTPB/Training_Course_Feedback/master/CFO.owl#recommendation -->

    <owl:Class rdf:about="https://raw.githubusercontent.com/GTPB/Training_Course_Feedback/master/CFO.owl#recommendation">
        <rdfs:subClassOf rdf:resource="https://raw.githubusercontent.com/GTPB/Training_Course_Feedback/master/CFO.owl#post_course"/>
        <rdfs:comment>A comment related to the participants willingness to recommend a training course</rdfs:comment>
        <rdfs:label>Recommendation</rdfs:label>
    </owl:Class>
    


    <!-- https://raw.githubusercontent.com/GTPB/Training_Course_Feedback/master/CFO.owl#references -->

    <owl:Class rdf:about="https://raw.githubusercontent.com/GTPB/Training_Course_Feedback/master/CFO.owl#references">
        <rdfs:subClassOf rdf:resource="https://raw.githubusercontent.com/GTPB/Training_Course_Feedback/master/CFO.owl#educational_content"/>
        <rdfs:comment>A comment related to the references recommended in a training course</rdfs:comment>
        <rdfs:label>References</rdfs:label>
    </owl:Class>
    


    <!-- https://raw.githubusercontent.com/GTPB/Training_Course_Feedback/master/CFO.owl#registration -->

    <owl:Class rdf:about="https://raw.githubusercontent.com/GTPB/Training_Course_Feedback/master/CFO.owl#registration">
        <rdfs:subClassOf rdf:resource="https://raw.githubusercontent.com/GTPB/Training_Course_Feedback/master/CFO.owl#course_logistics"/>
        <rdfs:comment>A subject related to the registration process of a training course</rdfs:comment>
        <rdfs:label>Registration</rdfs:label>
    </owl:Class>
    


    <!-- https://raw.githubusercontent.com/GTPB/Training_Course_Feedback/master/CFO.owl#relevance -->

    <owl:Class rdf:about="https://raw.githubusercontent.com/GTPB/Training_Course_Feedback/master/CFO.owl#relevance">
        <rdfs:subClassOf rdf:resource="https://raw.githubusercontent.com/GTPB/Training_Course_Feedback/master/CFO.owl#tag_descriptor"/>
    </owl:Class>
    


    <!-- https://raw.githubusercontent.com/GTPB/Training_Course_Feedback/master/CFO.owl#reminder -->

    <owl:Class rdf:about="https://raw.githubusercontent.com/GTPB/Training_Course_Feedback/master/CFO.owl#reminder">
        <rdfs:subClassOf rdf:resource="https://raw.githubusercontent.com/GTPB/Training_Course_Feedback/master/CFO.owl#announcement"/>
        <rdfs:comment>A comment related to the provision of a reminder notice for a training course event</rdfs:comment>
        <rdfs:label>Reminder</rdfs:label>
    </owl:Class>
    


    <!-- https://raw.githubusercontent.com/GTPB/Training_Course_Feedback/master/CFO.owl#resources -->

    <owl:Class rdf:about="https://raw.githubusercontent.com/GTPB/Training_Course_Feedback/master/CFO.owl#resources">
        <rdfs:subClassOf rdf:resource="https://raw.githubusercontent.com/GTPB/Training_Course_Feedback/master/CFO.owl#course_design_and_delivery"/>
        <rdfs:comment>A subject related to the resources used to facilitate a training course</rdfs:comment>
        <rdfs:label>Resources</rdfs:label>
    </owl:Class>
    


    <!-- https://raw.githubusercontent.com/GTPB/Training_Course_Feedback/master/CFO.owl#review -->

    <owl:Class rdf:about="https://raw.githubusercontent.com/GTPB/Training_Course_Feedback/master/CFO.owl#review">
        <rdfs:subClassOf rdf:resource="https://raw.githubusercontent.com/GTPB/Training_Course_Feedback/master/CFO.owl#impact"/>
        <rdfs:comment>The course consisted in an opportunity to review concepts learned in the past</rdfs:comment>
        <rdfs:label>Review</rdfs:label>
    </owl:Class>
    


    <!-- https://raw.githubusercontent.com/GTPB/Training_Course_Feedback/master/CFO.owl#scope -->

    <owl:Class rdf:about="https://raw.githubusercontent.com/GTPB/Training_Course_Feedback/master/CFO.owl#scope">
        <rdfs:subClassOf rdf:resource="https://raw.githubusercontent.com/GTPB/Training_Course_Feedback/master/CFO.owl#course_design_and_delivery"/>
        <rdfs:comment>A comment related to the topic extent covered in a training course</rdfs:comment>
        <rdfs:label>Course scope</rdfs:label>
    </owl:Class>
    


    <!-- https://raw.githubusercontent.com/GTPB/Training_Course_Feedback/master/CFO.owl#screens -->

    <owl:Class rdf:about="https://raw.githubusercontent.com/GTPB/Training_Course_Feedback/master/CFO.owl#screens">
        <rdfs:subClassOf rdf:resource="https://raw.githubusercontent.com/GTPB/Training_Course_Feedback/master/CFO.owl#computers"/>
        <rdfs:comment>A comment related to the screens of the computers in a training course</rdfs:comment>
        <rdfs:label>Screens</rdfs:label>
    </owl:Class>
    


    <!-- https://raw.githubusercontent.com/GTPB/Training_Course_Feedback/master/CFO.owl#selection -->

    <owl:Class rdf:about="https://raw.githubusercontent.com/GTPB/Training_Course_Feedback/master/CFO.owl#selection">
        <rdfs:subClassOf rdf:resource="https://raw.githubusercontent.com/GTPB/Training_Course_Feedback/master/CFO.owl#tag_descriptor"/>
    </owl:Class>
    


    <!-- https://raw.githubusercontent.com/GTPB/Training_Course_Feedback/master/CFO.owl#self_assessment -->

    <owl:Class rdf:about="https://raw.githubusercontent.com/GTPB/Training_Course_Feedback/master/CFO.owl#self_assessment">
        <rdfs:subClassOf rdf:resource="https://raw.githubusercontent.com/GTPB/Training_Course_Feedback/master/CFO.owl#post_course"/>
        <rdfs:comment>A subject related to the skills that the participant believe to have gained in participating in a training course</rdfs:comment>
        <rdfs:label>Self-assessment</rdfs:label>
    </owl:Class>
    


    <!-- https://raw.githubusercontent.com/GTPB/Training_Course_Feedback/master/CFO.owl#sequence -->

    <owl:Class rdf:about="https://raw.githubusercontent.com/GTPB/Training_Course_Feedback/master/CFO.owl#sequence">
        <rdfs:subClassOf rdf:resource="https://raw.githubusercontent.com/GTPB/Training_Course_Feedback/master/CFO.owl#tag_descriptor"/>
    </owl:Class>
    


    <!-- https://raw.githubusercontent.com/GTPB/Training_Course_Feedback/master/CFO.owl#servers -->

    <owl:Class rdf:about="https://raw.githubusercontent.com/GTPB/Training_Course_Feedback/master/CFO.owl#servers">
        <rdfs:subClassOf rdf:resource="https://raw.githubusercontent.com/GTPB/Training_Course_Feedback/master/CFO.owl#equipment"/>
        <rdfs:comment>A comment related to the servers used in a training course</rdfs:comment>
        <rdfs:label>Servers</rdfs:label>
    </owl:Class>
    


    <!-- https://raw.githubusercontent.com/GTPB/Training_Course_Feedback/master/CFO.owl#shuffling_pairs -->

    <owl:Class rdf:about="https://raw.githubusercontent.com/GTPB/Training_Course_Feedback/master/CFO.owl#shuffling_pairs">
        <rdfs:subClassOf rdf:resource="https://raw.githubusercontent.com/GTPB/Training_Course_Feedback/master/CFO.owl#implementation"/>
        <rdfs:comment>A comment related to the use of the shuffling pairs technique in a training room</rdfs:comment>
        <rdfs:label>Shuffling-pairs</rdfs:label>
    </owl:Class>
    


    <!-- https://raw.githubusercontent.com/GTPB/Training_Course_Feedback/master/CFO.owl#simulated_data -->

    <owl:Class rdf:about="https://raw.githubusercontent.com/GTPB/Training_Course_Feedback/master/CFO.owl#simulated_data">
        <rdfs:subClassOf rdf:resource="https://raw.githubusercontent.com/GTPB/Training_Course_Feedback/master/CFO.owl#dataset"/>
        <rdfs:comment>A comment related to the use of simulated data to cover the theme in a training course</rdfs:comment>
        <rdfs:label>Simulated data</rdfs:label>
    </owl:Class>
    


    <!-- https://raw.githubusercontent.com/GTPB/Training_Course_Feedback/master/CFO.owl#social -->

    <owl:Class rdf:about="https://raw.githubusercontent.com/GTPB/Training_Course_Feedback/master/CFO.owl#social">
        <rdfs:subClassOf rdf:resource="https://raw.githubusercontent.com/GTPB/Training_Course_Feedback/master/CFO.owl#participant_support"/>
        <rdfs:comment>A comment related to the activities of social engagement facilitated outside of the context of the training room in a training course</rdfs:comment>
        <rdfs:label>Social</rdfs:label>
    </owl:Class>
    


    <!-- https://raw.githubusercontent.com/GTPB/Training_Course_Feedback/master/CFO.owl#social_event -->

    <owl:Class rdf:about="https://raw.githubusercontent.com/GTPB/Training_Course_Feedback/master/CFO.owl#social_event">
        <rdfs:subClassOf rdf:resource="https://raw.githubusercontent.com/GTPB/Training_Course_Feedback/master/CFO.owl#social"/>
        <rdfs:comment>A comment related to the promotion and organization of a event (e.g. dinner) during the timespan of a training course</rdfs:comment>
        <rdfs:label>Social event</rdfs:label>
    </owl:Class>
    


    <!-- https://raw.githubusercontent.com/GTPB/Training_Course_Feedback/master/CFO.owl#software -->

    <owl:Class rdf:about="https://raw.githubusercontent.com/GTPB/Training_Course_Feedback/master/CFO.owl#software">
        <rdfs:subClassOf rdf:resource="https://raw.githubusercontent.com/GTPB/Training_Course_Feedback/master/CFO.owl#tools"/>
        <rdfs:comment>A comment related to the software tool selected to deploy the theme in a training course</rdfs:comment>
        <rdfs:label>Software</rdfs:label>
    </owl:Class>
    


    <!-- https://raw.githubusercontent.com/GTPB/Training_Course_Feedback/master/CFO.owl#some -->

    <owl:Class rdf:about="https://raw.githubusercontent.com/GTPB/Training_Course_Feedback/master/CFO.owl#some">
        <rdfs:subClassOf rdf:resource="https://raw.githubusercontent.com/GTPB/Training_Course_Feedback/master/CFO.owl#tag_qualifier"/>
    </owl:Class>
    


    <!-- https://raw.githubusercontent.com/GTPB/Training_Course_Feedback/master/CFO.owl#space -->

    <owl:Class rdf:about="https://raw.githubusercontent.com/GTPB/Training_Course_Feedback/master/CFO.owl#space">
        <rdfs:subClassOf rdf:resource="https://raw.githubusercontent.com/GTPB/Training_Course_Feedback/master/CFO.owl#training_room"/>
        <rdfs:comment>A comment related to the space distribution of the training room where a training course takes place</rdfs:comment>
        <rdfs:label>Space</rdfs:label>
    </owl:Class>
    


    <!-- https://raw.githubusercontent.com/GTPB/Training_Course_Feedback/master/CFO.owl#staff -->

    <owl:Class rdf:about="https://raw.githubusercontent.com/GTPB/Training_Course_Feedback/master/CFO.owl#staff">
        <rdfs:subClassOf rdf:resource="https://raw.githubusercontent.com/GTPB/Training_Course_Feedback/master/CFO.owl#resources"/>
        <rdfs:comment>A comment related to the staff involved in a training course</rdfs:comment>
        <rdfs:label>Staff</rdfs:label>
    </owl:Class>
    


    <!-- https://raw.githubusercontent.com/GTPB/Training_Course_Feedback/master/CFO.owl#statement -->

    <owl:Class rdf:about="https://raw.githubusercontent.com/GTPB/Training_Course_Feedback/master/CFO.owl#statement">
        <rdfs:subClassOf rdf:resource="https://raw.githubusercontent.com/GTPB/Training_Course_Feedback/master/CFO.owl#post_course"/>
        <rdfs:comment>A comment related to what the participant perceived to have learned in a training course</rdfs:comment>
        <rdfs:label>Statement</rdfs:label>
    </owl:Class>
    


    <!-- https://raw.githubusercontent.com/GTPB/Training_Course_Feedback/master/CFO.owl#strategies -->

    <owl:Class rdf:about="https://raw.githubusercontent.com/GTPB/Training_Course_Feedback/master/CFO.owl#strategies">
        <rdfs:subClassOf rdf:resource="https://raw.githubusercontent.com/GTPB/Training_Course_Feedback/master/CFO.owl#course_design_and_delivery"/>
        <rdfs:comment>A subject related to the strategies designed and implemented in a training course</rdfs:comment>
        <rdfs:label>Strategies</rdfs:label>
    </owl:Class>
    


    <!-- https://raw.githubusercontent.com/GTPB/Training_Course_Feedback/master/CFO.owl#structure -->

    <owl:Class rdf:about="https://raw.githubusercontent.com/GTPB/Training_Course_Feedback/master/CFO.owl#structure">
        <rdfs:subClassOf rdf:resource="https://raw.githubusercontent.com/GTPB/Training_Course_Feedback/master/CFO.owl#course_design_and_delivery"/>
        <rdfs:comment>A comment related to the structure of a training course</rdfs:comment>
        <rdfs:label>Structure</rdfs:label>
    </owl:Class>
    


    <!-- https://raw.githubusercontent.com/GTPB/Training_Course_Feedback/master/CFO.owl#subject_area -->

    <owl:Class rdf:about="https://raw.githubusercontent.com/GTPB/Training_Course_Feedback/master/CFO.owl#subject_area">
        <rdfs:subClassOf rdf:resource="https://raw.githubusercontent.com/GTPB/Training_Course_Feedback/master/CFO.owl#future_course_theme"/>
        <rdfs:comment>A subject area about which the course theme of interest by the participant is comprised</rdfs:comment>
        <rdfs:label>Subject area</rdfs:label>
    </owl:Class>
    


    <!-- https://raw.githubusercontent.com/GTPB/Training_Course_Feedback/master/CFO.owl#subject_context -->

    <owl:Class rdf:about="https://raw.githubusercontent.com/GTPB/Training_Course_Feedback/master/CFO.owl#subject_context">
        <rdfs:subClassOf rdf:resource="https://raw.githubusercontent.com/GTPB/Training_Course_Feedback/master/CFO.owl#future_course_theme"/>
        <rdfs:comment>A particular theme context about which the participant would be interested in a future course</rdfs:comment>
        <rdfs:label>Subject context</rdfs:label>
    </owl:Class>
    


    <!-- https://raw.githubusercontent.com/GTPB/Training_Course_Feedback/master/CFO.owl#subject_level -->

    <owl:Class rdf:about="https://raw.githubusercontent.com/GTPB/Training_Course_Feedback/master/CFO.owl#subject_level">
        <rdfs:subClassOf rdf:resource="https://raw.githubusercontent.com/GTPB/Training_Course_Feedback/master/CFO.owl#future_course_theme"/>
        <rdfs:comment>The level about which the participant would be interested in exploring a theme in a future course</rdfs:comment>
        <rdfs:label>Subject level</rdfs:label>
    </owl:Class>
    


    <!-- https://raw.githubusercontent.com/GTPB/Training_Course_Feedback/master/CFO.owl#subject_tool -->

    <owl:Class rdf:about="https://raw.githubusercontent.com/GTPB/Training_Course_Feedback/master/CFO.owl#subject_tool">
        <rdfs:subClassOf rdf:resource="https://raw.githubusercontent.com/GTPB/Training_Course_Feedback/master/CFO.owl#future_course_theme"/>
        <rdfs:comment>A tool about which the participant would be interested in exploring a theme in a future course</rdfs:comment>
        <rdfs:label>Subject tool</rdfs:label>
    </owl:Class>
    


    <!-- https://raw.githubusercontent.com/GTPB/Training_Course_Feedback/master/CFO.owl#subject_topic -->

    <owl:Class rdf:about="https://raw.githubusercontent.com/GTPB/Training_Course_Feedback/master/CFO.owl#subject_topic">
        <rdfs:subClassOf rdf:resource="https://raw.githubusercontent.com/GTPB/Training_Course_Feedback/master/CFO.owl#future_course_theme"/>
        <rdfs:comment>A particular topic about which the participant is interested in a future course</rdfs:comment>
        <rdfs:label>Subject topic</rdfs:label>
    </owl:Class>
    


    <!-- https://raw.githubusercontent.com/GTPB/Training_Course_Feedback/master/CFO.owl#suggestion -->

    <owl:Class rdf:about="https://raw.githubusercontent.com/GTPB/Training_Course_Feedback/master/CFO.owl#suggestion">
        <rdfs:subClassOf rdf:resource="https://raw.githubusercontent.com/GTPB/Training_Course_Feedback/master/CFO.owl#tag_qualifier"/>
    </owl:Class>
    


    <!-- https://raw.githubusercontent.com/GTPB/Training_Course_Feedback/master/CFO.owl#sumative_assess -->

    <owl:Class rdf:about="https://raw.githubusercontent.com/GTPB/Training_Course_Feedback/master/CFO.owl#sumative_assess">
        <rdfs:subClassOf rdf:resource="https://raw.githubusercontent.com/GTPB/Training_Course_Feedback/master/CFO.owl#assessment_instruments"/>
        <rdfs:comment>A subject related to the sumative assessment of participant&apos;s learning effectiveness in a training course (e.g. exam, diploma)</rdfs:comment>
        <rdfs:label>Sumative assess</rdfs:label>
    </owl:Class>
    


    <!-- https://raw.githubusercontent.com/GTPB/Training_Course_Feedback/master/CFO.owl#tag_descriptor -->

    <owl:Class rdf:about="https://raw.githubusercontent.com/GTPB/Training_Course_Feedback/master/CFO.owl#tag_descriptor">
        <rdfs:subClassOf rdf:resource="https://raw.githubusercontent.com/GTPB/Training_Course_Feedback/master/CFO.owl#course_assessment"/>
        <rdfs:comment>A description related to the tag mentioned in the comment given by the participant in a training course</rdfs:comment>
        <rdfs:label>Tag descriptor</rdfs:label>
    </owl:Class>
    


    <!-- https://raw.githubusercontent.com/GTPB/Training_Course_Feedback/master/CFO.owl#tag_qualifier -->

    <owl:Class rdf:about="https://raw.githubusercontent.com/GTPB/Training_Course_Feedback/master/CFO.owl#tag_qualifier">
        <rdfs:subClassOf rdf:resource="https://raw.githubusercontent.com/GTPB/Training_Course_Feedback/master/CFO.owl#course_assessment"/>
        <rdfs:comment>A qualifier related to the tag mentioned in the comment given by the participant in a training course</rdfs:comment>
        <rdfs:label>Tag qualifier</rdfs:label>
    </owl:Class>
    


    <!-- https://raw.githubusercontent.com/GTPB/Training_Course_Feedback/master/CFO.owl#temperature -->

    <owl:Class rdf:about="https://raw.githubusercontent.com/GTPB/Training_Course_Feedback/master/CFO.owl#temperature">
        <rdfs:subClassOf rdf:resource="https://raw.githubusercontent.com/GTPB/Training_Course_Feedback/master/CFO.owl#climate"/>
        <rdfs:comment>A comment related to the climatization system and the temperature of the training room where a training course takes place</rdfs:comment>
        <rdfs:label>Temperature</rdfs:label>
    </owl:Class>
    


    <!-- https://raw.githubusercontent.com/GTPB/Training_Course_Feedback/master/CFO.owl#testimonial -->

    <owl:Class rdf:about="https://raw.githubusercontent.com/GTPB/Training_Course_Feedback/master/CFO.owl#testimonial">
        <rdfs:subClassOf rdf:resource="https://raw.githubusercontent.com/GTPB/Training_Course_Feedback/master/CFO.owl#post_course"/>
        <rdfs:comment>A comment related to the participant&apos; s overall experience and general appreciation about a training course</rdfs:comment>
        <rdfs:label>Testimonial</rdfs:label>
    </owl:Class>
    


    <!-- https://raw.githubusercontent.com/GTPB/Training_Course_Feedback/master/CFO.owl#theme_focus -->

    <owl:Class rdf:about="https://raw.githubusercontent.com/GTPB/Training_Course_Feedback/master/CFO.owl#theme_focus">
        <rdfs:subClassOf rdf:resource="https://raw.githubusercontent.com/GTPB/Training_Course_Feedback/master/CFO.owl#course_design_and_delivery"/>
        <rdfs:comment>A comment related to the focus concerning the subject area of a training course</rdfs:comment>
        <rdfs:label>Theme focus</rdfs:label>
    </owl:Class>
    


    <!-- https://raw.githubusercontent.com/GTPB/Training_Course_Feedback/master/CFO.owl#theoretical_practical -->

    <owl:Class rdf:about="https://raw.githubusercontent.com/GTPB/Training_Course_Feedback/master/CFO.owl#theoretical_practical">
        <rdfs:subClassOf rdf:resource="https://raw.githubusercontent.com/GTPB/Training_Course_Feedback/master/CFO.owl#activity"/>
        <rdfs:comment>A comment related to the relation between the theoretical and the practical components in a training course</rdfs:comment>
        <rdfs:label>Theoretical-practical</rdfs:label>
    </owl:Class>
    


    <!-- https://raw.githubusercontent.com/GTPB/Training_Course_Feedback/master/CFO.owl#time_frame -->

    <owl:Class rdf:about="https://raw.githubusercontent.com/GTPB/Training_Course_Feedback/master/CFO.owl#time_frame">
        <rdfs:subClassOf rdf:resource="https://raw.githubusercontent.com/GTPB/Training_Course_Feedback/master/CFO.owl#timetable"/>
        <rdfs:comment>A comment related to the daily schedule of a training course in terms of clock (i.e. start time and end time and period time)</rdfs:comment>
        <rdfs:label>Time frame</rdfs:label>
    </owl:Class>
    


    <!-- https://raw.githubusercontent.com/GTPB/Training_Course_Feedback/master/CFO.owl#time_management -->

    <owl:Class rdf:about="https://raw.githubusercontent.com/GTPB/Training_Course_Feedback/master/CFO.owl#time_management">
        <rdfs:subClassOf rdf:resource="https://raw.githubusercontent.com/GTPB/Training_Course_Feedback/master/CFO.owl#course_design_and_delivery"/>
        <rdfs:comment>A comment related to the time management of a training course</rdfs:comment>
        <rdfs:label>Time management</rdfs:label>
    </owl:Class>
    


    <!-- https://raw.githubusercontent.com/GTPB/Training_Course_Feedback/master/CFO.owl#time_slot -->

    <owl:Class rdf:about="https://raw.githubusercontent.com/GTPB/Training_Course_Feedback/master/CFO.owl#time_slot">
        <rdfs:subClassOf rdf:resource="https://raw.githubusercontent.com/GTPB/Training_Course_Feedback/master/CFO.owl#timetable"/>
        <rdfs:comment>A comment related to the time allocated for each section and the time distribution within each section (e.g. division in morning block, lunch break, afternoon block) in a training course</rdfs:comment>
        <rdfs:label>Time slot</rdfs:label>
    </owl:Class>
    


    <!-- https://raw.githubusercontent.com/GTPB/Training_Course_Feedback/master/CFO.owl#timetable -->

    <owl:Class rdf:about="https://raw.githubusercontent.com/GTPB/Training_Course_Feedback/master/CFO.owl#timetable">
        <rdfs:subClassOf rdf:resource="https://raw.githubusercontent.com/GTPB/Training_Course_Feedback/master/CFO.owl#course_design_and_delivery"/>
        <rdfs:comment>A comment related to the timetable of a training course</rdfs:comment>
        <rdfs:label>Timetable</rdfs:label>
    </owl:Class>
    


    <!-- https://raw.githubusercontent.com/GTPB/Training_Course_Feedback/master/CFO.owl#timing -->

    <owl:Class rdf:about="https://raw.githubusercontent.com/GTPB/Training_Course_Feedback/master/CFO.owl#timing">
        <rdfs:subClassOf rdf:resource="https://raw.githubusercontent.com/GTPB/Training_Course_Feedback/master/CFO.owl#tag_descriptor"/>
    </owl:Class>
    


    <!-- https://raw.githubusercontent.com/GTPB/Training_Course_Feedback/master/CFO.owl#title -->

    <owl:Class rdf:about="https://raw.githubusercontent.com/GTPB/Training_Course_Feedback/master/CFO.owl#title">
        <rdfs:subClassOf rdf:resource="https://raw.githubusercontent.com/GTPB/Training_Course_Feedback/master/CFO.owl#organization_centred"/>
        <rdfs:comment>A comment related to the name of the course</rdfs:comment>
    </owl:Class>
    


    <!-- https://raw.githubusercontent.com/GTPB/Training_Course_Feedback/master/CFO.owl#tools -->

    <owl:Class rdf:about="https://raw.githubusercontent.com/GTPB/Training_Course_Feedback/master/CFO.owl#tools">
        <rdfs:subClassOf rdf:resource="https://raw.githubusercontent.com/GTPB/Training_Course_Feedback/master/CFO.owl#instructional_instruments"/>
        <rdfs:comment>A comment related to the tool(s) and/or platform(s) selected to cover the theme in a training course</rdfs:comment>
        <rdfs:label>Tools</rdfs:label>
    </owl:Class>
    


    <!-- https://raw.githubusercontent.com/GTPB/Training_Course_Feedback/master/CFO.owl#top_down -->

    <owl:Class rdf:about="https://raw.githubusercontent.com/GTPB/Training_Course_Feedback/master/CFO.owl#top_down">
        <rdfs:subClassOf rdf:resource="https://raw.githubusercontent.com/GTPB/Training_Course_Feedback/master/CFO.owl#approach"/>
        <rdfs:comment>A comment related to the approach of covering a subject starting with the abstract concepts and working down the theme, step by step, to the specfic details in a training course</rdfs:comment>
        <rdfs:label>Top-down approach</rdfs:label>
    </owl:Class>
    


    <!-- https://raw.githubusercontent.com/GTPB/Training_Course_Feedback/master/CFO.owl#topics -->

    <owl:Class rdf:about="https://raw.githubusercontent.com/GTPB/Training_Course_Feedback/master/CFO.owl#topics">
        <rdfs:subClassOf rdf:resource="https://raw.githubusercontent.com/GTPB/Training_Course_Feedback/master/CFO.owl#structure"/>
        <rdfs:subClassOf rdf:resource="https://raw.githubusercontent.com/GTPB/Training_Course_Feedback/master/CFO.owl#time_management"/>
        <rdfs:comment>A comment related to the topics covered in a training course</rdfs:comment>
        <rdfs:label>Topics</rdfs:label>
    </owl:Class>
    


    <!-- https://raw.githubusercontent.com/GTPB/Training_Course_Feedback/master/CFO.owl#training_room -->

    <owl:Class rdf:about="https://raw.githubusercontent.com/GTPB/Training_Course_Feedback/master/CFO.owl#training_room">
        <rdfs:subClassOf rdf:resource="https://raw.githubusercontent.com/GTPB/Training_Course_Feedback/master/CFO.owl#resources"/>
        <rdfs:comment>A comment related to the comfort ot the training room where a training course takes place</rdfs:comment>
        <rdfs:label>Training room</rdfs:label>
    </owl:Class>
    


    <!-- https://raw.githubusercontent.com/GTPB/Training_Course_Feedback/master/CFO.owl#tutorials -->

    <owl:Class rdf:about="https://raw.githubusercontent.com/GTPB/Training_Course_Feedback/master/CFO.owl#tutorials">
        <rdfs:subClassOf rdf:resource="https://raw.githubusercontent.com/GTPB/Training_Course_Feedback/master/CFO.owl#materials"/>
        <rdfs:comment>A comment related to the tutorials and/or manual actively used in a training course</rdfs:comment>
        <rdfs:label>Tutorials</rdfs:label>
    </owl:Class>
    


    <!-- https://raw.githubusercontent.com/GTPB/Training_Course_Feedback/master/CFO.owl#tutoring -->

    <owl:Class rdf:about="https://raw.githubusercontent.com/GTPB/Training_Course_Feedback/master/CFO.owl#tutoring">
        <rdfs:subClassOf rdf:resource="https://raw.githubusercontent.com/GTPB/Training_Course_Feedback/master/CFO.owl#methods"/>
        <rdfs:comment>A comment related to the adoption of the tutoring model in a training course</rdfs:comment>
        <rdfs:label>Tutoring</rdfs:label>
    </owl:Class>
    


    <!-- https://raw.githubusercontent.com/GTPB/Training_Course_Feedback/master/CFO.owl#updated -->

    <owl:Class rdf:about="https://raw.githubusercontent.com/GTPB/Training_Course_Feedback/master/CFO.owl#updated">
        <rdfs:subClassOf rdf:resource="https://raw.githubusercontent.com/GTPB/Training_Course_Feedback/master/CFO.owl#testimonial"/>
        <rdfs:comment>The course was updated</rdfs:comment>
        <rdfs:label>Updated</rdfs:label>
    </owl:Class>
    


    <!-- https://raw.githubusercontent.com/GTPB/Training_Course_Feedback/master/CFO.owl#useful -->

    <owl:Class rdf:about="https://raw.githubusercontent.com/GTPB/Training_Course_Feedback/master/CFO.owl#useful">
        <rdfs:subClassOf rdf:resource="https://raw.githubusercontent.com/GTPB/Training_Course_Feedback/master/CFO.owl#impact"/>
        <rdfs:comment>The course was useful for the participant current and future interests</rdfs:comment>
        <rdfs:label>Useful</rdfs:label>
    </owl:Class>
    


    <!-- https://raw.githubusercontent.com/GTPB/Training_Course_Feedback/master/CFO.owl#variability -->

    <owl:Class rdf:about="https://raw.githubusercontent.com/GTPB/Training_Course_Feedback/master/CFO.owl#variability">
        <rdfs:subClassOf rdf:resource="https://raw.githubusercontent.com/GTPB/Training_Course_Feedback/master/CFO.owl#tag_descriptor"/>
    </owl:Class>
    


    <!-- https://raw.githubusercontent.com/GTPB/Training_Course_Feedback/master/CFO.owl#video_recording -->

    <owl:Class rdf:about="https://raw.githubusercontent.com/GTPB/Training_Course_Feedback/master/CFO.owl#video_recording">
        <rdfs:subClassOf rdf:resource="https://raw.githubusercontent.com/GTPB/Training_Course_Feedback/master/CFO.owl#auxiliary"/>
        <rdfs:comment>A comment related to the recording in video of a training course</rdfs:comment>
        <rdfs:label>Video recording</rdfs:label>
    </owl:Class>
    


    <!-- https://raw.githubusercontent.com/GTPB/Training_Course_Feedback/master/CFO.owl#visibility -->

    <owl:Class rdf:about="https://raw.githubusercontent.com/GTPB/Training_Course_Feedback/master/CFO.owl#visibility">
        <rdfs:subClassOf rdf:resource="https://raw.githubusercontent.com/GTPB/Training_Course_Feedback/master/CFO.owl#tag_descriptor"/>
    </owl:Class>
    


    <!-- https://raw.githubusercontent.com/GTPB/Training_Course_Feedback/master/CFO.owl#worthwhile -->

    <owl:Class rdf:about="https://raw.githubusercontent.com/GTPB/Training_Course_Feedback/master/CFO.owl#worthwhile">
        <rdfs:subClassOf rdf:resource="https://raw.githubusercontent.com/GTPB/Training_Course_Feedback/master/CFO.owl#impact"/>
        <rdfs:comment>The course was worth taken, even taking into account the potential constraints (like the fee or the not straightforward professional gain)</rdfs:comment>
        <rdfs:label>Worthwhile</rdfs:label>
    </owl:Class>
    


    <!-- https://raw.githubusercontent.com/GTPB/Training_Course_Feedback/master/CFO.owl#wrap_up -->

    <owl:Class rdf:about="https://raw.githubusercontent.com/GTPB/Training_Course_Feedback/master/CFO.owl#wrap_up">
        <rdfs:subClassOf rdf:resource="https://raw.githubusercontent.com/GTPB/Training_Course_Feedback/master/CFO.owl#content_scheme"/>
        <rdfs:comment>A comment related to the overview part of the content in a training course</rdfs:comment>
        <rdfs:label>Wrap-up</rdfs:label>
    </owl:Class>
</rdf:RDF>



<!-- Generated by the OWL API (version 4.5.6.2018-09-06T00:27:41Z) https://github.com/owlcs/owlapi -->

